7 apr

Master/ExoticInteger.v
@@ -10,71 +10,71 @@ Inductive ExoticZ : Type :=
 
 
 (* Add for ExoticZ *)
-Function succ' (k : ExoticZ) : ExoticZ :=
+Function eSucc (k : ExoticZ) : ExoticZ :=
 match k with
 | Zero' => Next Zero'
 | MinusOne => Zero'
 | Next Zero' => Next (Next Zero')
 | Next MinusOne => MinusOne
-| Next k' => Next (succ' k')
+| Next k' => Next (eSucc k')
 end.
 
-Function pred' (k : ExoticZ) : ExoticZ :=
+Function ePred (k : ExoticZ) : ExoticZ :=
 match k with
 | Zero' => MinusOne
 | MinusOne => Next MinusOne
 | Next Zero' => Zero'
 | Next MinusOne => Next (Next MinusOne)
-| Next k' => Next (pred' k')
+| Next k' => Next (ePred k')
 end.
 
-Function abs (k: ExoticZ) : nat :=
+Function eAbs (k: ExoticZ) : nat :=
 match k with
 | Zero'    => 0
 | MinusOne => 1
-| Next k'  => S (abs k')
+| Next k'  => S (eAbs k')
 end.
 
-Function pos (k: ExoticZ) : bool :=
+Function ePos (k: ExoticZ) : bool :=
 match k with
 | Zero'    => true
 | MinusOne => false
-| Next k'  => pos k'
+| Next k'  => ePos k'
 end.
 
-Definition add' (a b : ExoticZ) : ExoticZ :=
-match pos a with 
-| true  => map_n (abs a) succ' b
-| false => map_n (abs a) pred' b
+Definition eAdd (a b : ExoticZ) : ExoticZ :=
+match ePos a with 
+| true  => map_n (eAbs a) eSucc b
+| false => map_n (eAbs a) ePred b
 end.
 
-Lemma next_pos_is_same : forall z: ExoticZ, pos z = pos (Next z).
+Lemma next_pos_is_same : forall z: ExoticZ, ePos z = ePos (Next z).
 Proof.
   intros z. induction z; auto.
 Qed.
 
-Lemma if_pos_next_is_succ : forall z: ExoticZ, pos z = true -> Next z = succ' z.
+Lemma if_pos_next_is_succ : forall z: ExoticZ, ePos z = true -> Next z = eSucc z.
 Proof.
   intro z. induction z; auto.
   - intros H. cbn in *. discriminate H.
-  - intros H. assert (P: pos z = true) by (rewrite <- H; apply next_pos_is_same; auto).
+  - intros H. assert (P: ePos z = true) by (rewrite <- H; apply next_pos_is_same; auto).
     cbn. specialize (IHz P). rewrite <- IHz. destruct z; auto. cbn in P. discriminate.
 Qed.
 
-Lemma if_neg_next_is_pred : forall z: ExoticZ, pos z = false -> Next z = pred' z.
+Lemma if_neg_next_is_pred : forall z: ExoticZ, ePos z = false -> Next z = ePred z.
 Proof.
   intro z. induction z; auto.
   - intros H. cbn in *. discriminate H.
-  - intros H. assert (P: pos z = false) by (rewrite <- H; apply next_pos_is_same; auto).
+  - intros H. assert (P: ePos z = false) by (rewrite <- H; apply next_pos_is_same; auto).
     cbn. specialize (IHz P). rewrite <- IHz. destruct z; auto. cbn in P. discriminate.
 Qed.
 
-Theorem ExoticZ_ind' (P : ExoticZ -> Prop) (base: P Zero') (suc: forall z: ExoticZ, P z -> P (succ' z)) 
-  (pre: forall z: ExoticZ, P z -> P (pred' z)) : forall z: ExoticZ, P z.
+Theorem ExoticZ_ind' (P : ExoticZ -> Prop) (base: P Zero') (suc: forall z: ExoticZ, P z -> P (eSucc z)) 
+  (pre: forall z: ExoticZ, P z -> P (ePred z)) : forall z: ExoticZ, P z.
 Proof.
   intro z. induction z; auto.
   - apply (pre _ base).
-  - destruct (pos z) eqn:pos.
+  - destruct (ePos z) eqn:pos.
     + rewrite (if_pos_next_is_succ z pos). apply (suc _ IHz).
     + rewrite (if_neg_next_is_pred z pos). apply (pre _ IHz).
 Qed.
@@ -87,9 +87,9 @@ Definition h (n: ExoticZ) : Z :=
 match n with
 | Zero'    => Zero
 | MinusOne => Neg O
-| Next n'  => if pos n' 
-              then Pos (abs n')
-              else Neg (abs n')
+| Next n'  => if ePos n' 
+              then Pos (eAbs n')
+              else Neg (eAbs n')
 end.
 
 Definition h_inv (n: Z) : ExoticZ :=
@@ -102,34 +102,34 @@ end.
 
 
 
-Lemma abs_for_map_n : forall n: nat, abs (map_n n Next Zero') = n.
+Lemma abs_for_map_n : forall n: nat, eAbs (map_n n Next Zero') = n.
 Proof.
   intros n. induction n; auto. cbn. f_equal. assumption.
 Qed.
 
-Lemma abs_for_map_n' : forall n: nat, abs (map_n n Next MinusOne) = S n.
+Lemma abs_for_map_n' : forall n: nat, eAbs (map_n n Next MinusOne) = S n.
 Proof.
   intros n. induction n; auto. cbn. f_equal. assumption.
 Qed.
 
-Lemma pos_for_map_n : forall n: nat, pos (map_n n Next Zero') = true.
+Lemma pos_for_map_n : forall n: nat, ePos (map_n n Next Zero') = true.
 Proof.
   intros n. induction n; auto.
 Qed.
 
-Lemma pos_for_map_n' : forall n: nat, pos (map_n n Next MinusOne) = false.
+Lemma pos_for_map_n' : forall n: nat, ePos (map_n n Next MinusOne) = false.
 Proof.
   intros n. induction n; auto.
 Qed.
 
-Lemma map_n_abs_pos : forall n: ExoticZ, pos n = true -> map_n (abs n) Next Zero' = n.
+Lemma map_n_abs_pos : forall n: ExoticZ, ePos n = true -> map_n (eAbs n) Next Zero' = n.
 Proof.
   intros n H. induction n; auto.
   - cbn in *. discriminate.
   - cbn in *. f_equal. apply IHn. assumption. 
 Qed.
 
-Lemma map_n_abs_neg : forall n: ExoticZ, pos n = false -> map_n (abs n) Next MinusOne = Next n.
+Lemma map_n_abs_neg : forall n: ExoticZ, ePos n = false -> map_n (eAbs n) Next MinusOne = Next n.
 Proof.
   intros n H. induction n; auto.
   - cbn in *. discriminate.
@@ -148,7 +148,7 @@ Qed.
 
 Theorem h_bijection' : forall x : ExoticZ, h_inv (h x) = x.
 Proof.
-  intros x. destruct x; auto. cbn. destruct (pos x) eqn:P; cbn.
+  intros x. destruct x; auto. cbn. destruct (ePos x) eqn:P; cbn.
   - f_equal. now apply map_n_abs_pos.
   - now apply map_n_abs_neg.
 Qed.
@@ -165,97 +165,97 @@ Qed.
 
 
 
-Lemma pred'_for_pos : forall x : ExoticZ, pos x = true -> pred' (Next x) = x.
+Lemma ePred_for_pos : forall x : ExoticZ, ePos x = true -> ePred (Next x) = x.
 Proof.
   intros x P. induction x; cbn in *; [auto | discriminate |]. specialize (IHx P).
   now rewrite IHx.
 Qed.
 
-Lemma succ'_for_neg : forall x : ExoticZ, pos x = false -> succ' (Next x) = x.
+Lemma eSucc_for_neg : forall x : ExoticZ, ePos x = false -> eSucc (Next x) = x.
 Proof.
   intros x P. induction x; cbn in *; [discriminate | auto |]. specialize (IHx P).
   now rewrite IHx.
 Qed.
 
-Lemma pred'_for_neg : forall x : ExoticZ, pos x = false -> pred' x = Next x.
+Lemma ePred_for_neg : forall x : ExoticZ, ePos x = false -> ePred x = Next x.
 Proof.
   intros x P. induction x; cbn in *; [discriminate | auto |]. specialize (IHx P).
   rewrite IHx. destruct x; [| auto | auto]. cbn in *. discriminate.
 Qed.
 
-Lemma succ'_for_pos : forall x : ExoticZ, pos x = true -> succ' x = Next x.
+Lemma eSucc_for_pos : forall x : ExoticZ, ePos x = true -> eSucc x = Next x.
 Proof.
   intros x P. induction x; cbn in *; [auto | discriminate |]. specialize (IHx P).
   rewrite IHx. destruct x; [auto | | auto]. cbn in *. discriminate.
 Qed.
 
-Lemma succ'_pred': forall k : ExoticZ, succ' (pred' k) = k.
+Lemma eSucc_ePred: forall k : ExoticZ, eSucc (ePred k) = k.
 Proof.
-  intros x. functional induction (pred' x); cbn; [auto | auto | auto | auto |]. 
-  rewrite IHe. functional induction (pred' k'); cbn; auto. contradiction.
+  intros x. functional induction (ePred x); cbn; [auto | auto | auto | auto |]. 
+  rewrite IHe. functional induction (ePred k'); cbn; auto. contradiction.
 Qed.
 
-Lemma pred'_succ' : forall k : ExoticZ, pred' (succ' k) = k.
+Lemma ePred_eSucc : forall k : ExoticZ, ePred (eSucc k) = k.
 Proof.
-  intros k; functional induction (succ' k); cbn; [auto | auto | auto | auto |]. 
-  rewrite IHe. functional induction (succ' k'); cbn in *; auto.
+  intros k; functional induction (eSucc k); cbn; [auto | auto | auto | auto |]. 
+  rewrite IHe. functional induction (eSucc k'); cbn in *; auto.
   contradiction.
 Qed.
 
-Lemma pred_h : forall x: ExoticZ, pred (h x) = h (pred' x).
+Lemma pred_h : forall x: ExoticZ, pred (h x) = h (ePred x).
 Proof.
-  intro x. destruct (pos x) eqn:P; destruct x; auto; cbn in P.
-  - rewrite pred'_for_pos; auto. cbn. rewrite P.
+  intro x. destruct (ePos x) eqn:P; destruct x; auto; cbn in P.
+  - rewrite ePred_for_pos; auto. cbn. rewrite P.
     destruct x; cbn in *; [auto | discriminate|]. now rewrite P.
-  - rewrite pred'_for_neg; auto. cbn. now rewrite P.
+  - rewrite ePred_for_neg; auto. cbn. now rewrite P.
 Qed.
 
-Lemma succ_h : forall x: ExoticZ, succ (h x) = h (succ' x).
+Lemma succ_h : forall x: ExoticZ, succ (h x) = h (eSucc x).
 Proof.
-  intro x. destruct (pos x) eqn:P; destruct x; auto; cbn in P.
-  - rewrite succ'_for_pos; auto. cbn. now rewrite P.
-  - rewrite succ'_for_neg; auto. cbn. rewrite P. 
+  intro x. destruct (ePos x) eqn:P; destruct x; auto; cbn in P.
+  - rewrite eSucc_for_pos; auto. cbn. now rewrite P.
+  - rewrite eSucc_for_neg; auto. cbn. rewrite P. 
     destruct x; cbn in *; [auto | auto |]. now rewrite P.
 Qed.
 
-Lemma add'_l_succ' : forall x y: ExoticZ, add' (succ' x) y = succ' (add' x y).
+Lemma eAdd_l_eSucc : forall x y: ExoticZ, eAdd (eSucc x) y = eSucc (eAdd x y).
 Proof.
   intros x y. induction y using ExoticZ_ind'.
-  - destruct x; auto. unfold add'. destruct (pos x) eqn:P.
-    + rewrite succ'_for_pos; auto. cbn. now rewrite P.
-    + rewrite succ'_for_neg; auto. cbn. now rewrite P, succ'_pred'.
+  - destruct x; auto. unfold eAdd. destruct (ePos x) eqn:P.
+    + rewrite eSucc_for_pos; auto. cbn. now rewrite P.
+    + rewrite eSucc_for_neg; auto. cbn. now rewrite P, eSucc_ePred.
   - destruct x; auto.
-    + cbn. now  rewrite succ'_pred'.
-    + unfold add'. destruct (pos x) eqn:P.
-      * rewrite succ'_for_pos; auto. cbn. now rewrite P.
-      * rewrite succ'_for_neg; auto. cbn. now rewrite P, succ'_pred'.
+    + cbn. now  rewrite eSucc_ePred.
+    + unfold eAdd. destruct (ePos x) eqn:P.
+      * rewrite eSucc_for_pos; auto. cbn. now rewrite P.
+      * rewrite eSucc_for_neg; auto. cbn. now rewrite P, eSucc_ePred.
   - destruct x; auto.
-    + cbn. now rewrite succ'_pred'.
-    + unfold add'. destruct (pos x) eqn:P.
-      * rewrite succ'_for_pos; auto. cbn. now rewrite P.
-      * rewrite succ'_for_neg; auto. cbn. now rewrite P, succ'_pred'.
+    + cbn. now rewrite eSucc_ePred.
+    + unfold eAdd. destruct (ePos x) eqn:P.
+      * rewrite eSucc_for_pos; auto. cbn. now rewrite P.
+      * rewrite eSucc_for_neg; auto. cbn. now rewrite P, eSucc_ePred.
 Qed.
 
-Lemma add'_l_pred' : forall x y: ExoticZ, add' (pred' x) y = pred' (add' x y).
+Lemma eAdd_l_ePred : forall x y: ExoticZ, eAdd (ePred x) y = ePred (eAdd x y).
 Proof.
   intros x y. induction y using ExoticZ_ind'.
-  - destruct x; auto. unfold add'. destruct (pos x) eqn:P.
-    + rewrite pred'_for_pos; auto. cbn. now rewrite P, pred'_succ'.
-    + rewrite pred'_for_neg; auto. cbn. now rewrite P.
-  - destruct x; auto. unfold add'. destruct (pos x) eqn:P.
-    + rewrite pred'_for_pos; auto. cbn. now rewrite P, pred'_succ'.
-    + rewrite pred'_for_neg; auto. cbn. now rewrite P.
-  - destruct x; auto. unfold add'. destruct (pos x) eqn:P.
-    + rewrite pred'_for_pos; auto. cbn. now rewrite P, pred'_succ'.
-    + rewrite pred'_for_neg; auto. cbn. now rewrite P.
+  - destruct x; auto. unfold eAdd. destruct (ePos x) eqn:P.
+    + rewrite ePred_for_pos; auto. cbn. now rewrite P, ePred_eSucc.
+    + rewrite ePred_for_neg; auto. cbn. now rewrite P.
+  - destruct x; auto. unfold eAdd. destruct (ePos x) eqn:P.
+    + rewrite ePred_for_pos; auto. cbn. now rewrite P, ePred_eSucc.
+    + rewrite ePred_for_neg; auto. cbn. now rewrite P.
+  - destruct x; auto. unfold eAdd. destruct (ePos x) eqn:P.
+    + rewrite ePred_for_pos; auto. cbn. now rewrite P, ePred_eSucc.
+    + rewrite ePred_for_neg; auto. cbn. now rewrite P.
 Qed.
 
 (* Homomorphism of algebraic structures *)
-Theorem Z_ExoticZ_homo : forall x y: ExoticZ, add (h x) (h y) = h (add' x y).
+Theorem Z_ExoticZ_homo : forall x y: ExoticZ, add (h x) (h y) = h (eAdd x y).
 Proof.
   intros x y. induction x using ExoticZ_ind'; [auto|..].
-  - now rewrite add'_l_succ', <- succ_h, <- succ_h, <- IHx, add_l_succ.
-  - now rewrite add'_l_pred', <- pred_h, <- pred_h, <- IHx, add_l_pred.
+  - now rewrite eAdd_l_eSucc, <- succ_h, <- succ_h, <- IHx, add_l_succ.
+  - now rewrite eAdd_l_ePred, <- pred_h, <- pred_h, <- IHx, add_l_pred.
 Qed.
 
 
