Master/FreeGroup.v
@@ -4,53 +4,20 @@ Require Import Coq.Lists.List.
 Require Import StrictProp.
 Import ListNotations.
 
-Class Group (A : Type) := GroupDef {
-  zero      : A;
-  op        : A -> A -> A;
-  inv       : A -> A;
-  eqf       : A -> A -> bool;
-  left_id   : forall x: A, op zero x = x;
-  right_id  : forall x: A, op x zero = x;
-  left_inv  : forall x: A, op (inv x) x = zero;
-  right_inv : forall x: A, op x (inv x) = zero;
-  op_assoc  : forall x y z: A, op (op x y) z = op x (op y z);
-  eqf_eq    : forall x y, reflect (x = y) (eqf x y)
-}.
+Require Import Lib.Algebra.
+Require Import Lib.Normalization.
+Require Import Lib.EqDec.
 
-Lemma eqf_refl {A: Type} `{Group A} (x : A) : eqf x x = true.
+
+Class EqGroup (A : Type) `{E: EqDec A} `{G: Group A} := {}.
+
+Global Instance EqGroup_def {A: Type} `{E: EqDec A} `{G: Group A} : EqGroup A.
 Proof.
-  destruct (eqf_eq x x); auto.
 Qed.
 
-Definition eqf_true_iff {A: Type} `{Group A} {x y: A} : eqf x y = true <-> x = y.
-Proof.
-  destruct (eqf_eq x y); split; auto. intros F. discriminate.
-Qed.
+Definition CanonFreeGroup (A: Type) `{EqGroup A} := list (bool*A).
 
-Definition eqf_false_iff {A: Type} `{Group A} {x y: A} : eqf x y = false <-> x <> y.
-Proof.
-  split.
-  - intros H0 H1. subst. rewrite eqf_refl in H0. discriminate.
-  - intros H0. destruct (eqf_eq x y); auto. subst. contradiction.
-Defined.
-
-Lemma eqf_sym {A: Type} `{Group A} (x y: A) : eqf x y = eqf y x.
-Proof.
-  destruct (eqf_eq x y).
-  - subst. rewrite eqf_refl. auto.
-  - assert (y <> x) by (apply not_eq_sym; auto). rewrite <- eqf_false_iff in H0.
-    rewrite H0. auto.
-Qed.
-
-
-(* Notation "a @ b" := (op a b) (at level 51, right associativity).
-Notation "c ^" := (inv c) (at level 40). *)
-
-Definition sub {A: Type} `{Group A} (x y: A) := op x (inv y).
-
-Definition CanonFreeGroup (A: Type) `{Group A} := list (bool*A).
-
-Fixpoint normalize {A: Type} `{Group A} (x: CanonFreeGroup A) :=
+Fixpoint normalize {A: Type} `{EqGroup A} (x: CanonFreeGroup A) :=
 match x with
 | [] => []
 | (b, v) :: x' => 
@@ -62,72 +29,66 @@ match x with
     end
 end.
 
-Inductive Normalized {A: Type} `{Group A} : CanonFreeGroup A -> Prop :=
+Inductive Normalized {A: Type} `{EqGroup A} : CanonFreeGroup A -> Prop :=
 | NNil   : Normalized []
 | NSingl : forall (b : bool) (v : A), Normalized [(b, v)]
 | NCons  : forall (b b': bool) (v v' : A) (x: CanonFreeGroup A), 
             v <> v' \/ b = b' -> Normalized ((b', v') :: x) ->
             Normalized ((b, v) :: (b', v') :: x).
 
-Inductive NonEmptyFreeGroup (A: Type) `{Group A} :=
-| Singl  : bool -> A -> NonEmptyFreeGroup A
-| Switch : forall x: A, Squash (x <> zero) -> NonEmptyFreeGroup A -> NonEmptyFreeGroup A
-| Stay   : A -> NonEmptyFreeGroup A -> NonEmptyFreeGroup A.
 
-Arguments Switch {A H}.
-Arguments Stay {A H}.
-Arguments Singl {A H}.
 
-Definition FreeGroup (A: Type) `{Group A} := option (NonEmptyFreeGroup A).
+Inductive NEQuotFreeGroup (A: Type) `{EqGroup A} :=
+| Singl  : bool -> A -> NEQuotFreeGroup A
+| Switch : forall x: A, Squash (x <> zero) -> NEQuotFreeGroup A -> NEQuotFreeGroup A
+| Stay   : A -> NEQuotFreeGroup A -> NEQuotFreeGroup A.
 
-Print reflect.
+Arguments Switch {A E G H}.
+Arguments Stay {A E G H}.
+Arguments Singl {A E G H}.
 
-Fixpoint to_uniq' {A: Type} `{Group A} (b : bool) (v: A) (x: CanonFreeGroup A) : NonEmptyFreeGroup A :=
+Definition QuotFreeGroup (A: Type) `{EqGroup A} := option (NEQuotFreeGroup A).
+
+Fixpoint to_quot' {A: Type} `{EqGroup A} (b : bool) (v: A) (x: CanonFreeGroup A) : NEQuotFreeGroup A :=
 match x with 
 | []             => Singl b v
 | (b', v') :: x' => if eqb b b' 
-                      then Stay (sub v v') (to_uniq' b' v' x')
-                      else match eqf_eq (sub v v') zero with
-                           | ReflectF _ p => Switch (sub v v') (squash p) (to_uniq' b' v' x')
+                      then Stay (sub v v') (to_quot' b' v' x')
+                      else match eqf_leibniz (sub v v') zero with
+                           | ReflectF _ p => Switch (sub v v') (squash p) (to_quot' b' v' x')
                            | _  => (Singl b v) (* invalid *)
                            end
 end.
 
-Definition to_uniq {A: Type} `{Group A} (x: CanonFreeGroup A) : FreeGroup A :=
+Definition to_quot {A: Type} `{EqGroup A} (x: CanonFreeGroup A) : QuotFreeGroup A :=
 match x with
 | [] => None
-| (b, v) :: x' => Some (to_uniq' b v x')
+| (b, v) :: x' => Some (to_quot' b v x')
 end.
 
-Fixpoint to_canon' {A: Type} `{Group A} (x: NonEmptyFreeGroup A) : CanonFreeGroup A :=
+Definition all_to_quot {A: Type} `{EqGroup A} (x: CanonFreeGroup A) : QuotFreeGroup A :=
+to_quot (normalize x).
+
+Fixpoint to_canon' {A: Type} `{EqGroup A} (x: NEQuotFreeGroup A) : bool * A * list (bool*A) :=
 match x with 
-| Singl b v     => [(b, v)]
+| Singl b v     => ((b, v), [])
 | Stay v x'     => match to_canon' x' with
-                   | [] => [(true, v)] (* invalid *)
-                   | (b, v') :: y => (b, op v v') :: (b, v') :: y
+                   | ((b, v'), y)  => ((b, op v v'), (b, v') :: y)
                    end
 | Switch v _ x' => match to_canon' x' with
-                   | [] => [(true, v)] (* invalid *)
-                   | (b, v') :: y => (negb b, op v v') :: (b, v') :: y
+                   | ((b, v'), y)  => ((negb b, op v v'), (b, v') :: y)
                    end
 end.
 
-Definition to_canon {A: Type} `{Group A} (x: FreeGroup A) : CanonFreeGroup A :=
+Definition to_canon {A: Type} `{EqGroup A} (x: QuotFreeGroup A) : CanonFreeGroup A :=
 match x with
 | None => []
-| Some x' => to_canon' x'
+| Some x' => let (h, t) := to_canon' x' in h :: t
 end.
 
-Lemma op_sub {A: Type} `{Group A} (x y : A) : op (sub x y) y = x.
-Proof.
-  unfold sub. rewrite op_assoc. rewrite left_inv. rewrite right_id. auto.
-Qed.
 
-Lemma sub_op {A: Type} `{Group A} (x y : A) : sub (op x y) y = x.
-Proof.
-  unfold sub. rewrite op_assoc. rewrite right_inv. rewrite right_id. auto.
-Qed.
 
+(* Ancilary lemmas *)
 Lemma squash_not_refl {A : Type} (x: A) (P: Prop) : Squash (x <> x) -> P.
 Proof.
   intros H. apply sEmpty_ind. apply (Squash_sind (x <> x)); auto.
@@ -151,328 +112,18 @@ Proof.
   - intros H. subst. destruct y; auto.
 Qed.
 
-Lemma group_equation_l_simp {A: Type} `{Group A} (a b c : A) : op a b = op a c -> b = c.
+Lemma group_squash_non_zero {A: Type} `{EqGroup A} (x : A) : Squash (x <> zero) -> x <> zero.
 Proof.
-  intro H0. assert (op (inv a) (op a b) = op (inv a) (op a c)).
-  - rewrite H0. auto.
-  - rewrite <- op_assoc, <- op_assoc, left_inv, left_id, left_id in H1. auto.
+  intros H0. destruct (eqf_leibniz x zero); auto. subst. apply (squash_not_refl zero). auto.
 Qed.
 
-Lemma group_equation_r_simp {A: Type} `{Group A} (a b c : A) : op a c = op b c -> a = b.
-Proof.
-  intro H0. assert (op (op a c) (inv c) = op (op b c) (inv c)).
-  - rewrite H0. auto.
-  - rewrite op_assoc, op_assoc, right_inv, right_id, right_id in H1. auto.
-Qed.
-
-Lemma sub_inv_uniq {A: Type} `{Group A} (x y: A) : sub x y = zero -> x = y.
-Proof.
-  unfold sub. rewrite <- (right_inv y). intros H0. 
-  apply group_equation_r_simp with (c := inv y). auto.
-Qed.
-
-Theorem free_group_epi_canon {A: Type} `{Group A} (x: FreeGroup A) : 
-  to_uniq (to_canon x) = x.
-Proof.
-  destruct x as [x |]; auto. induction x; auto.
-  - cbn in *. destruct (to_canon' x0); inversion IHx. destruct p. cbn in *. 
-    inversion IHx. subst. rewrite eqb_negb1, sub_op. destruct (eqf_eq x zero); auto.
-    subst. apply (squash_not_refl zero); auto.
-  - cbn in *. destruct (to_canon' x); inversion IHx. destruct p. cbn in *.
-    inversion IHx. subst. rewrite eqb_reflx, sub_op. auto.
-Qed.
-
-Theorem canon_epi_free_group {A: Type} `{Group A} (x: CanonFreeGroup A) : 
-  Normalized x -> to_canon (to_uniq x) = x.
-Proof.
-  intros N. induction N; auto. cbn in *. destruct H0 as [v_neq | b_neq].
-  - destruct (eqb b b') eqn:b_eq.
-    + cbn. rewrite IHN, op_sub. f_equal. f_equal. symmetry. apply eqb_prop. auto.
-    + destruct (eqf_eq (sub v v') zero).
-      * assert (v = v') by (apply sub_inv_uniq; auto). contradiction.
-      * cbn. rewrite IHN, op_sub. f_equal. f_equal. symmetry. apply not_eqb_is_neg. auto.
-  - subst. rewrite eqb_reflx. cbn. rewrite IHN, op_sub. auto.
-Qed.
-
-Lemma to_canon'_not_nil {A: Type} `{Group A} (x: NonEmptyFreeGroup A) : to_canon' x <> nil.
-Proof.
-  intros H0. destruct x; cbn in *.
-  - inversion H0.
-  - destruct (to_canon' x0).
-    + inversion H0.
-    + destruct p. inversion H0.
-  - destruct (to_canon' x).
-    + inversion H0.
-    + destruct p. inversion H0.
-Qed.
-
-Lemma group_add_non_zero {A: Type} `{Group A} (x y : A) : x <> zero -> op x y <> y.
-Proof.
-  intros H0 H1. apply H0. apply group_equation_r_simp with (c := op y (inv y)).
-  rewrite <- op_assoc, H1, right_inv, left_id. auto.
-Qed.
-
-Lemma group_squash_non_zero {A: Type} `{Group A} (x : A) : Squash (x <> zero) -> x <> zero.
-Proof.
-  intros H0. destruct (eqf_eq x zero); auto. subst. apply (squash_not_refl zero). auto.
-Qed. 
-
-Theorem free_group_is_normal {A: Type} `{Group A} (x: FreeGroup A) : Normalized (to_canon x).
-Proof.
-  destruct x as [x |].
-  - induction x.
-    + cbn. constructor.
-    + dependent destruction IHx.
-      * assert (to_canon (Some x0) <> []) by (apply to_canon'_not_nil). rewrite x in H0.
-        contradiction.
-      * cbn in *. rewrite <- x. constructor; constructor. apply group_add_non_zero. 
-        apply group_squash_non_zero. auto.
-      * cbn in *. rewrite <- x. constructor.
-        -- left. apply group_add_non_zero. apply group_squash_non_zero. auto.
-        -- constructor; auto.
-    + dependent destruction IHx.
-      * assert (to_canon (Some x0) <> []) by (apply to_canon'_not_nil). rewrite x in H0.
-        contradiction.
-      * cbn in *. rewrite <- x. constructor; try right; constructor.
-      * cbn in *. rewrite <- x. constructor; try right; constructor; auto.
-  - cbn. constructor.
-Qed.
-
-Definition option_bind {A B: Type} (x: option A) (f: A -> option B) : option B :=
-  match x with
-  | None => None
-  | Some x' => f x'
-  end. 
-
-Fixpoint fg_hd' {A: Type} `{Group A} (x: NonEmptyFreeGroup A) : bool * A :=
-  match x with 
-  | Singl b v => (b, v)
-  | Stay v x' => let (b', v') := fg_hd' x' in (b', op v v')
-  | Switch v _ x' => let (b', v') := fg_hd' x' in (negb b', op v v')
-  end.
-
-Definition fg_hd {A: Type} `{Group A} (x: FreeGroup A) : option (bool * A) :=
-  option_map fg_hd' x.
-
-Theorem fg_hd_for_canon {A: Type} `{Group A} (x: CanonFreeGroup A) :
-  Normalized x -> hd_error x = fg_hd (to_uniq x).
-Proof.
-  intros H0. induction H0; auto. cbn in *. f_equal. inversion IHNormalized. destruct H0.
-  - destruct (eqb b b') eqn:e.
-    + cbn. rewrite <- H3, op_sub. rewrite eqb_true_iff in e. f_equal; auto.
-    + destruct (eqf_eq (sub v v') zero); auto. cbn. rewrite <- H3, op_sub. f_equal.
-      apply not_eqb_is_neg. auto.
-  - subst. rewrite eqb_reflx. cbn. rewrite <- H3, op_sub. auto.
-Qed.
-
-Definition fq_tail' {A: Type} `{Group A} (x: NonEmptyFreeGroup A) : FreeGroup A :=
-  match x with 
-  | Singl _ _     => None
-  | Stay _ x'     => Some x'
-  | Switch _ _ x' => Some x'
-  end.
-
-Definition fg_tail {A: Type} `{Group A} (x: FreeGroup A) : FreeGroup A :=
-  option_bind x fq_tail'.
-
-Definition fg_cons' {A: Type} `{Group A} (b: bool) (v: A) (x: NonEmptyFreeGroup A) : 
-   FreeGroup A :=
-    let (b', v') := fg_hd' x in 
-      if eqb b b'
-      then Some (Stay (sub v v') x)
-      else match eqf_eq (sub v v') zero with
-           | ReflectT _ _ => fq_tail' x
-           | ReflectF _ p => Some (Switch (sub v v') (squash p) x)
-           end.
-
-Definition fg_cons'2 {A: Type} `{Group A} (p : bool * A) (x: NonEmptyFreeGroup A) :=
-  let (b, v) := p in fg_cons' b v x.
-
-Definition fg_cons {A: Type} `{Group A} (b: bool) (v: A) (x: FreeGroup A) : FreeGroup A :=
-  match x with
-  | None => Some (Singl b v)
-  | Some x' => fg_cons' b v x'
-  end.
-
-Definition fg_cons2 {A: Type} `{Group A} (p: bool * A) (x: FreeGroup A) : FreeGroup A := 
-  let (b, v) := p in fg_cons b v x.
- 
-Definition elem_inv {A: Type} (x : bool * A) := let (b, v) := x in (negb b, v).
-
-Theorem inv_elem_cons_is_tail {A: Type} `{Group A} (x: NonEmptyFreeGroup A) :
-  fg_cons'2 (elem_inv (fg_hd' x)) x = fq_tail' x.
-Proof.
-  destruct (fg_hd' x) eqn:hd. destruct x; cbn.
-  - inversion hd. unfold sub. rewrite eqb_negb1, right_inv.
-    destruct (eqf_eq zero zero); auto. contradiction.
-  - unfold fg_cons', sub. rewrite hd, eqb_negb1, right_inv. 
-    destruct (eqf_eq zero zero); auto. contradiction.
-  - unfold fg_cons', sub. rewrite hd, eqb_negb1, right_inv. 
-    destruct (eqf_eq zero zero); auto. contradiction.
-Qed.
-
-Definition canon_cons {A: Type} `{Group A} (b: bool) (v: A) (x: CanonFreeGroup A) :
-  CanonFreeGroup A :=
-  match x with
-  | [] => [(b, v)]
-  | (b', v') :: t => if negb (eqf v v') || eqb b b'
-                     then (b, v) :: (b', v') :: t
-                     else t
-  end.
-
-Fixpoint canon_concat {A: Type} `{Group A} (x y: CanonFreeGroup A) : CanonFreeGroup A :=
-  match x with
-  | []           => y
-  | (b, v) :: x' => canon_cons b v (canon_concat x' y)
-  end.
-
-Theorem concat_norm {A: Type} `{Group A} (x y: CanonFreeGroup A) : 
-  Normalized x -> Normalized y -> Normalized (canon_concat x y).
-Proof.
-  intros Nx Ny. induction Nx; auto.
-  - cbn. destruct Ny; unfold canon_cons.
-    + constructor.
-    + destruct (negb (eqf v v0) || eqb b b0 ) eqn:e; constructor.
-      * rewrite orb_true_iff, eqb_true_iff, negb_true_iff, eqf_false_iff in e. auto.
-      * constructor.
-    + destruct (negb (eqf v v0) || eqb b b0) eqn:e; auto. constructor.
-      * rewrite orb_true_iff, eqb_true_iff, negb_true_iff, eqf_false_iff in e. auto.
-      * constructor; auto.
-  - cbn. destruct (canon_concat x y) eqn:c; unfold canon_cons in *.
-    + assert (negb (eqf v v') || eqb b b' = true).
-      * rewrite orb_true_iff, eqb_true_iff, negb_true_iff, eqf_false_iff. auto.
-      * rewrite H1. constructor; auto. constructor.
-    + destruct p. cbn in *. rewrite c in IHNx. destruct (negb (eqf v' a) || eqb b' b0) eqn:e.
-      * assert (negb (eqf v v') || eqb b b' = true); unfold canon_cons in *.
-        -- rewrite orb_true_iff, eqb_true_iff, negb_true_iff, eqf_false_iff. auto.
-        -- rewrite H1. rewrite e in IHNx. constructor; auto.
-      * cbn in *. destruct c0; try constructor. destruct p.
-        destruct (negb (eqf v a0) || eqb b b1) eqn:e1; unfold canon_cons in *; rewrite e in IHNx.
-        -- constructor; auto.
-           rewrite orb_true_iff, eqb_true_iff, negb_true_iff, eqf_false_iff in e1. auto.
-        -- dependent destruction IHNx; auto. constructor.
-Qed.
-
-Fixpoint fg_concat' {A: Type} `{Group A} (x: NonEmptyFreeGroup A) 
-  (y: FreeGroup A) : FreeGroup A :=
-  match x with
-  | Singl b v     => fg_cons b v y
-  | Stay _ x'     => fg_cons2 (fg_hd' x) (fg_concat' x' y)
-  | Switch _ _ x' => fg_cons2 (fg_hd' x) (fg_concat' x' y)
-  end.
-
-Definition fg_concat {A: Type} `{Group A} (x y: FreeGroup A) : FreeGroup A :=
-  match x with
-  | None => y
-  | Some x' => fg_concat' x' y
-  end.
-
-Lemma eqf_sub_not_zero {A: Type} `{Group A} (x y: A) : sub x y <> zero <-> eqf x y = false.
+Lemma eqf_sub_not_zero {A: Type} `{EqGroup A} (x y: A) : sub x y <> zero <-> eqf x y = false.
 Proof.
   unfold sub. split.
-  - intros H0. destruct (eqf_eq x y); auto. subst. rewrite right_inv in H0. 
+  - intros H0. destruct (eqf_leibniz x y); [|auto]. subst. rewrite r_op_inv in H0. 
     contradiction.
-  - intros H0 H1. assert (x = y) by (apply sub_inv_uniq; auto). subst.
+  - intros H0 H1. assert (x = y) by (apply sub_zero_uniq; auto). subst.
     rewrite eqf_refl in H0. discriminate.
-Qed.
-
-Theorem free_canon_hd'_izo {A: Type} `{Group A} (x: NonEmptyFreeGroup A) :
-  Some (fg_hd' x) = hd_error (to_canon (Some x)).
-Proof.
-  induction x; auto.
-  - cbn in *. destruct (to_canon' x0) eqn:e.
-    + exfalso. apply (to_canon'_not_nil x0). auto.
-    + destruct p. cbn in *. inversion IHx. rewrite H1. auto.
-  - cbn in *. destruct (to_canon' x) eqn:e.
-    + exfalso. apply (to_canon'_not_nil x). auto.
-    + destruct p. cbn in *. inversion IHx. rewrite H1. auto.
-Qed.
-
-Theorem free_canon_hd_izo {A: Type} `{Group A} (x: FreeGroup A) :
-  fg_hd x = hd_error (to_canon x).
-Proof.
-  destruct x as [x |]; auto. cbn. apply free_canon_hd'_izo.
-Qed.
-
-Theorem free_canon_cons_izo {A: Type} `{Group A} (b: bool) (v: A) (x: FreeGroup A) :
-  to_canon (fg_cons b v x) = canon_cons b v (to_canon x).
-Proof.
-  destruct x as [x |]; auto. unfold canon_cons. destruct x.
-  - cbn. destruct (eqb b b0) eqn:e.
-    + cbn. rewrite orb_true_r, op_sub. rewrite eqb_true_iff in e. subst. auto.
-    + destruct (eqf_eq (sub v a) zero).
-      * assert (v = a) by (apply sub_inv_uniq; auto). subst.
-        rewrite eqf_refl. cbn. auto.
-      * cbn. rewrite eqf_sub_not_zero in n. rewrite n, op_sub. cbn.
-        assert (negb b0 = b) by (symmetry; apply not_eqb_is_neg; auto). 
-        subst. auto.
-  - cbn. destruct (to_canon' x0) eqn:c.
-    + exfalso. apply (to_canon'_not_nil x0). auto.
-    + destruct p. unfold fg_cons'. cbn. assert (hd_eq : fg_hd' x0 = (b0, a)).
-      { apply some_eq. rewrite free_canon_hd'_izo. cbn. rewrite c. auto. }
-      rewrite hd_eq. destruct (eqb b (negb b0)) eqn:eb.
-      * cbn. rewrite orb_true_r, c, op_sub. rewrite eqb_true_iff in eb. subst.
-        auto.
-      * destruct (eqf_eq (sub v (op x a))).
-        -- assert (v = (op x a)) by (apply sub_inv_uniq; auto). subst.
-          rewrite eqf_refl. cbn. auto.
-        -- cbn. rewrite eqf_sub_not_zero in n. rewrite n, c. unfold sub. cbn.
-           rewrite (op_assoc  v (inv (op x a))), left_inv, right_id, negb_involutive.
-           f_equal. rewrite eqb_not_neg in eb. subst. auto.
-  - cbn. destruct (to_canon' x) eqn:c.
-    + exfalso. apply (to_canon'_not_nil x). auto.
-    + destruct p. unfold fg_cons'. cbn. assert (hd_eq : fg_hd' x = (b0, a0)).
-      { apply some_eq. rewrite free_canon_hd'_izo. cbn. rewrite c. auto. }
-      rewrite hd_eq. destruct (eqb b b0) eqn:eb.
-      * cbn. rewrite orb_true_r, c, op_sub. rewrite eqb_true_iff in eb. subst.
-        auto.
-      * destruct (eqf_eq (sub v (op a a0))).
-        -- assert (v = (op a a0)) by (apply sub_inv_uniq; auto). subst.
-          rewrite eqf_refl. cbn. auto.
-        -- cbn. rewrite eqf_sub_not_zero in n. rewrite n, c. unfold sub. cbn.
-           rewrite (op_assoc  v (inv (op a a0))), left_inv, right_id.
-           f_equal. assert (b = negb b0) by (apply not_eqb_is_neg; auto).
-           subst. auto.
-Qed.
-
-Theorem free_canon_concat_izo {A: Type} `{Group A} (x y: FreeGroup A) :
-  to_canon (fg_concat x y) = canon_concat (to_canon x) (to_canon y).
-Proof.
-  destruct x as [x |]; auto. cbn. induction x.
-  - cbn. apply free_canon_cons_izo.
-  - cbn. destruct (to_canon' x0) eqn:c.
-    + exfalso. apply (to_canon'_not_nil x0). auto.
-    + destruct p. assert (hd_eq : fg_hd' x0 = (b, a)).
-      { apply some_eq. rewrite free_canon_hd'_izo. cbn. rewrite c. auto. }
-      rewrite hd_eq. cbn in *. rewrite <- IHx. apply free_canon_cons_izo.
-  - cbn. destruct (to_canon' x) eqn:c.
-    + exfalso. apply (to_canon'_not_nil x). auto.
-    + destruct p. assert (hd_eq : fg_hd' x = (b, a0)).
-      { apply some_eq. rewrite free_canon_hd'_izo. cbn. rewrite c. auto. }
-      rewrite hd_eq. cbn in *. rewrite <- IHx. apply free_canon_cons_izo.
-Qed.
-
-Fixpoint canon_apinv {A: Type} `{Group A} (x y: CanonFreeGroup A) :=
-  match x with
-  | [] => y
-  | (b, v) :: x' => canon_apinv x' (cons (negb b, v) y)
-  end.
-
-Definition canon_inv {A: Type} `{Group A} (x: CanonFreeGroup A) := canon_apinv x [].
-
-Fixpoint canon_append {A: Type} `{Group A} (b: bool) (v: A) (x: CanonFreeGroup A) :=
-  match x with
-  | [] => [(b, v)]
-  | [(b', v')] => if negb (eqf v v') || eqb b b'
-                     then [(b', v'); (b, v)]
-                     else []
-  | h :: x' => h :: (canon_append b v x')
-  end.
-
-Theorem group_inv_inv {A: Type} `{Group A} (x: A) : inv (inv x) = x.
-Proof.
-  rewrite <- (right_id (inv (inv x))), <- (left_inv x), <- (op_assoc), left_inv, left_id.
-  auto.
 Qed.
 
 Lemma eqb_sym (x y : bool) : eqb x y = eqb y x.
@@ -490,55 +141,365 @@ Proof.
   intros H H0. destruct x, y, z; auto; cbn in *; discriminate.
 Qed.
 
-Lemma condition_iff {A: Type} `{Group A} (b b': bool) (v v': A) :
+Lemma condition_iff {A: Type} `{EqGroup A} (b b': bool) (v v': A) :
   v <> v' \/ b = b' <-> negb (eqf v v') || eqb b b' = true.
 Proof.
   split.
   - intros [|].
-    + rewrite <- eqf_false_iff in H0. rewrite H0. auto.
+    + rewrite not_eqf_iff in H0. rewrite H0. auto.
     + subst. rewrite eqb_reflx, orb_true_r. auto.
   - intro H0. rewrite orb_true_iff, negb_true_iff in H0. destruct H0.
-    + left. rewrite <- eqf_false_iff. auto.
+    + left. rewrite not_eqf_iff. auto.
     + right. apply eqb_prop. auto.
 Qed.
 
-Lemma condition_false_iff {A: Type} `{Group A} (b b': bool) (v v': A) :
+Lemma condition_iff' {A: Type} `{EqGroup A} (b b': bool) (v v': A) :
+  v <> v' \/ b = b' <-> eqf v v' && xorb b b' = false.
+Proof.
+  split.
+  - intros [|].
+    + rewrite not_eqf_iff in H0. rewrite H0. auto.
+    + subst. rewrite xorb_nilpotent, andb_false_r. auto.
+  - intro H0. rewrite andb_false_iff in H0. destruct H0.
+    + left. rewrite not_eqf_iff. auto.
+    + right. apply xorb_eq. auto.
+Qed.
+
+
+Lemma condition_false_iff {A: Type} `{EqGroup A} (b b': bool) (v v': A) :
   v = v' /\ b = negb b' <-> negb (eqf v v') || eqb b b' = false.
 Proof.
   split.
   - intros []. subst. rewrite eqf_refl, eqb_negb1. auto.
   - intro H0. rewrite orb_false_iff, negb_false_iff in H0. destruct H0. split.
-    + rewrite <- eqf_true_iff. auto.
+    + rewrite eqf_iff. auto.
     + destruct b, b'; auto; cbn in *; try discriminate.
 Qed.
 
-Lemma append_for_normalized {A: Type} `{Group A} (b: bool) (v: A) (x : CanonFreeGroup A) : 
+
+Lemma eqb_neg_izo (x y : bool) : eqb (negb x) (negb y) = eqb x y.
+Proof.
+  destruct x, y; auto.
+Qed.
+
+
+(* normalization lemmas *)
+
+Lemma normalized_without_head {A: Type} `{EqGroup A} (b: bool) (v: A) (x: CanonFreeGroup A) :
+  Normalized ((b, v) :: x) -> Normalized x.
+Proof.
+  intros Nx. destruct x; [constructor|].
+  destruct p as (b', v'). now dependent destruction Nx.
+Qed.
+
+Lemma concat_normalized_l {A: Type} `{EqGroup A} (x y: CanonFreeGroup A) :
+  Normalized (x ++ y) -> Normalized x.
+Proof.
+  destruct x as [| (b, v)]; [constructor|].
+  revert b v. induction x as [| (b', v')]; intros b v H0; [constructor|].
+  dependent destruction H0. constructor; auto.
+Qed.
+
+Lemma concat_normalized_r {A: Type} `{EqGroup A} (x y: CanonFreeGroup A) :
+  Normalized (x ++ y) -> Normalized y.
+Proof.
+  induction x as [| (b, v)]; [auto|].
+  intros H0. apply IHx. rewrite <- app_comm_cons in H0.
+  now apply (normalized_without_head b v).
+Qed.
+
+Theorem normalize_normalizes {A: Type} `{EqGroup A} (x: CanonFreeGroup A) :
+  Normalized (normalize x).
+Proof.
+  induction x as [|(b & v) x]; [constructor | ].
+  cbn in *. destruct (normalize x) as [|(b' & v') x']; [constructor|].
+  destruct (eqf v v' && xorb b b') eqn:e.
+  - now apply (normalized_without_head b' v').
+  - constructor; [|auto]. now apply condition_iff'.
+Qed.
+
+Theorem normalize_is_id_for_normalized {A: Type} `{EqGroup A} (x: CanonFreeGroup A) :
+  Normalized x -> normalize x = x.
+Proof.
+  intros Nx. induction Nx; [auto | auto |]. rewrite condition_iff' in H0.
+  cbn in *. destruct (normalize x) as [| (b'' & v'') l].
+  - now rewrite H0, IHNx.
+  - now rewrite IHNx, H0.  
+Qed.
+
+Theorem normalize_idempotent {A: Type} `{EqGroup A} :
+  normalzation normalize.
+Proof.
+  intros x. symmetry. apply normalize_is_id_for_normalized.
+  apply normalize_normalizes.
+Qed.
+
+
+
+
+(* to_quot and to_canon lemmas *)
+Theorem quot_epi_canon {A: Type} `{EqGroup A} (x: QuotFreeGroup A) : 
+  to_quot (to_canon x) = x.
+Proof.
+  destruct x as [x |]; auto. induction x; [auto|..]; cbn in *.
+  - destruct (to_canon' x0) as [[b  v] l]. cbn in *. 
+    inversion IHx. subst. rewrite eqb_negb1, sub_op. 
+    destruct (eqf_leibniz x zero); [|auto]. subst. now apply (squash_not_refl zero).
+  - destruct (to_canon' x) as [[b  v] l]. cbn in *.
+    inversion IHx. subst. now rewrite eqb_reflx, sub_op.
+Qed.
+
+Theorem canon_epi_quot {A: Type} `{EqGroup A} (x: CanonFreeGroup A) : 
+  Normalized x -> to_canon (to_quot x) = x.
+Proof.
+  intros N. induction N; [auto | auto |]. cbn in *. destruct H0 as [v_neq | b_neq].
+  - destruct (eqb b b') eqn:b_eq.
+    + cbn. destruct (to_canon' (to_quot' b' v' x)) as [[b'' v''] l]. 
+      inversion IHN. subst. rewrite op_sub. f_equal. f_equal. symmetry. 
+      now apply eqb_prop.
+    + destruct (eqf_leibniz (sub v v') zero).
+      * assert (v = v') by (apply sub_zero_uniq; auto). contradiction.
+      * cbn. destruct (to_canon' (to_quot' b' v' x)) as [[b'' v''] l]. 
+        inversion IHN; subst. rewrite op_sub. f_equal. f_equal. symmetry. 
+        now apply not_eqb_is_neg.
+  - subst. rewrite eqb_reflx. cbn. destruct (to_canon' (to_quot' b' v' x)) as [[b'' v''] l]. 
+    inversion IHN; subst. now rewrite op_sub.
+Qed.
+
+Lemma to_canon_not_nil {A: Type} `{EqGroup A} (x: NEQuotFreeGroup A) : to_canon (Some x) <> nil.
+Proof.
+  intros H0. destruct x; cbn in *; [inversion H0|..].
+  - destruct (to_canon' x0) as [[b v] l]. inversion H0.
+  - destruct (to_canon' x) as [[b v] l]. inversion H0.
+Qed.
+
+Theorem quot_is_normal {A: Type} `{EqGroup A} (x: QuotFreeGroup A) : Normalized (to_canon x).
+Proof.
+  destruct x as [x |]; cbn; [|constructor]. induction x.
+  - cbn. constructor.
+  - dependent destruction IHx; cbn in *.
+    + assert (to_canon (Some x0) <> []) by (apply to_canon_not_nil). rewrite x in H0.
+      contradiction.
+    + destruct (to_canon' x0) as [[b' v'] l]. inversion x; subst.
+      constructor; constructor. apply add_is_non_zero. apply group_squash_non_zero. auto.
+    + destruct (to_canon' x0) as [[b'' v''] l]. inversion x; subst. constructor.
+      * left. apply add_is_non_zero. now apply group_squash_non_zero.
+      * now constructor.
+  - dependent destruction IHx; cbn in *.
+    + assert (to_canon (Some x0) <> []) by (apply to_canon_not_nil). rewrite x in H0.
+      contradiction.
+    + destruct (to_canon' x0) as [[b' v'] l]. inversion x; subst. 
+      constructor; [right|]; constructor.
+    + destruct (to_canon' x1) as [[b'' v''] l]. inversion x; subst. 
+      constructor; [right|]; now constructor.
+Qed.
+
+
+
+
+(* Canon concat definition *)
+
+Definition canon_cons {A: Type} `{EqGroup A} (b: bool) (v: A) (x: CanonFreeGroup A) :
+  CanonFreeGroup A :=
+  match x with
+  | [] => [(b, v)]
+  | (b', v') :: t => if negb (eqf v v') || eqb b b'
+                     then (b, v) :: (b', v') :: t
+                     else t
+  end.
+
+Fixpoint canon_concat {A: Type} `{EqGroup A} (x y: CanonFreeGroup A) : CanonFreeGroup A :=
+  match x with
+  | []           => y
+  | (b, v) :: x' => canon_cons b v (canon_concat x' y)
+  end.
+
+Theorem concat_norm {A: Type} `{EqGroup A} (x y: CanonFreeGroup A) : 
+  Normalized x -> Normalized y -> Normalized (canon_concat x y).
+Proof.
+  intros Nx Ny. induction Nx; [auto | ..]; cbn.
+  - destruct Ny; unfold canon_cons.
+    + constructor.
+    + destruct (negb (eqf v v0) || eqb b b0 ) eqn:e; constructor;
+      [now rewrite orb_true_iff, eqb_true_iff, negb_true_iff, <-not_eqf_iff in e | constructor].
+    + destruct (negb (eqf v v0) || eqb b b0) eqn:e; auto. constructor;
+      [now rewrite orb_true_iff, eqb_true_iff, negb_true_iff, <-not_eqf_iff in e | now constructor].
+  - assert (negb (eqf v v') || eqb b b' = true) by
+    now rewrite orb_true_iff, eqb_true_iff, negb_true_iff, <-not_eqf_iff.
+    destruct (canon_concat x y) as [|(b'' & v'') l] eqn:c; unfold canon_cons in *.
+    + rewrite H1. constructor; [auto | constructor].
+    + cbn in *. rewrite c in *. unfold canon_cons in *. 
+      destruct (negb (eqf v' v'') || eqb b' b'') eqn:e.
+      * assert (negb (eqf v v') || eqb b b' = true) by
+        now rewrite orb_true_iff, eqb_true_iff, negb_true_iff, <-not_eqf_iff.
+        rewrite H2. constructor; auto.
+      * cbn in *. destruct c; try constructor. destruct l as [| (b''' & v''')]; [constructor|]. 
+        destruct (negb (eqf v v''') || eqb b b''') eqn:e1.
+        -- constructor; [now rewrite orb_true_iff, eqb_true_iff, negb_true_iff, <-not_eqf_iff in e1 | auto].
+        -- dependent destruction IHNx; [constructor | auto].
+Qed.
+
+
+
+
+(* Quot concat homomorphism *)
+Fixpoint quot_hd' {A: Type} `{EqGroup A} (x: NEQuotFreeGroup A) : bool * A :=
+  match x with 
+  | Singl b v => (b, v)
+  | Stay v x' => let (b', v') := quot_hd' x' in (b', op v v')
+  | Switch v _ x' => let (b', v') := quot_hd' x' in (negb b', op v v')
+  end.
+
+Definition fq_tail' {A: Type} `{EqGroup A} (x: NEQuotFreeGroup A) : QuotFreeGroup A :=
+  match x with 
+  | Singl _ _     => None
+  | Stay _ x'     => Some x'
+  | Switch _ _ x' => Some x'
+  end.
+
+Definition quot_cons' {A: Type} `{EqGroup A} (b: bool) (v: A) (x: NEQuotFreeGroup A) : 
+   QuotFreeGroup A :=
+    let (b', v') := quot_hd' x in 
+      if eqb b b'
+      then Some (Stay (sub v v') x)
+      else match eqf_leibniz (sub v v') zero with
+           | ReflectT _ _ => fq_tail' x
+           | ReflectF _ p => Some (Switch (sub v v') (squash p) x)
+           end.
+
+Definition quot_cons {A: Type} `{EqGroup A} (b: bool) (v: A) (x: QuotFreeGroup A) : QuotFreeGroup A :=
+  match x with
+  | None => Some (Singl b v)
+  | Some x' => quot_cons' b v x'
+  end.
+
+Definition quot_cons2 {A: Type} `{EqGroup A} (p: bool * A) (x: QuotFreeGroup A) : QuotFreeGroup A := 
+  let (b, v) := p in quot_cons b v x.
+
+Fixpoint quot_concat' {A: Type} `{EqGroup A} (x: NEQuotFreeGroup A) 
+  (y: QuotFreeGroup A) : QuotFreeGroup A :=
+  match x with
+  | Singl b v     => quot_cons b v y
+  | Stay _ x'     => quot_cons2 (quot_hd' x) (quot_concat' x' y)
+  | Switch _ _ x' => quot_cons2 (quot_hd' x) (quot_concat' x' y)
+  end.
+
+Definition quot_concat {A: Type} `{EqGroup A} (x y: QuotFreeGroup A) : QuotFreeGroup A :=
+  match x with
+  | None => y
+  | Some x' => quot_concat' x' y
+  end.
+
+Theorem quot_canon_hd {A: Type} `{EqGroup A} (x: NEQuotFreeGroup A) :
+  Some (quot_hd' x) = hd_error (to_canon (Some x)).
+Proof.
+  induction x; [auto|..].
+  - cbn in *. destruct (to_canon' x0) as [[b v] l] eqn:e.
+    cbn in *. inversion IHx. now rewrite H1.
+  - cbn in *. destruct (to_canon' x) as [[b v] l] eqn:e.
+    cbn in *. inversion IHx. now rewrite H1.
+Qed.
+
+Theorem quot_canon_cons_homomorphism {A: Type} `{EqGroup A} (b: bool) (v: A) (x: QuotFreeGroup A) :
+  to_canon (quot_cons b v x) = canon_cons b v (to_canon x).
+Proof.
+  destruct x as [x |]; auto. unfold canon_cons. destruct x as [b' v' | v' p x' | v' x'].
+  - cbn. destruct (eqb b b') eqn:e.
+    + cbn. rewrite orb_true_r, op_sub. f_equal. f_equal. symmetry. now apply eqb_prop.
+    + destruct (eqf_leibniz (sub v v') zero).
+      * assert (v = v') by now apply sub_zero_uniq. subst.
+        rewrite eqf_refl. auto.
+      * cbn. rewrite eqf_sub_not_zero in n. rewrite n, op_sub. cbn. f_equal. f_equal.
+        assert (negb b' = b) by (symmetry; now apply not_eqb_is_neg). auto. 
+  - cbn. destruct (to_canon' x') as [[b'' v''] l] eqn:c.
+    unfold quot_cons'. cbn. assert (hd_eq : quot_hd' x' = (b'', v'')).
+    { apply some_eq. rewrite quot_canon_hd. cbn. now rewrite c. }
+    rewrite hd_eq. destruct (eqb b (negb b'')) eqn:eb.
+    + cbn. rewrite eqb_true_iff in eb; subst. now rewrite orb_true_r, c, op_sub. 
+    + destruct (eqf_leibniz (sub v (op v' v''))).
+      * assert (v = (op v' v'')) by (apply sub_zero_uniq; auto). subst.
+        cbn. now rewrite eqf_refl, c.
+      * cbn. rewrite eqf_sub_not_zero in n. rewrite n, c. unfold sub. cbn.
+        rewrite (op_assoc  v (inv (op v' v''))), l_op_inv, r_op_id, negb_involutive.
+        f_equal. rewrite eqb_not_neg in eb. subst. auto.
+  - cbn. destruct (to_canon' x') as [[b'' v''] l] eqn:c.
+    unfold quot_cons'. cbn. assert (hd_eq : quot_hd' x' = (b'', v'')).
+    { apply some_eq. rewrite quot_canon_hd. cbn. now rewrite c. }
+    rewrite hd_eq. destruct (eqb b b'') eqn:eb.
+    + cbn. rewrite eqb_true_iff in eb; subst. now rewrite orb_true_r, c, op_sub. 
+    + destruct (eqf_leibniz (sub v (op v' v''))).
+      * assert (v = (op v' v'')) by (apply sub_zero_uniq; auto). subst.
+        cbn. now rewrite eqf_refl, c.
+      * cbn. rewrite eqf_sub_not_zero in n. rewrite n, c. unfold sub. cbn.
+        rewrite (op_assoc  v (inv (op v' v''))), l_op_inv, r_op_id.
+        f_equal. assert (b = negb b'') by (apply not_eqb_is_neg; auto).
+        subst. auto.
+Qed.
+
+Theorem quot_canon_concat_homomorphism {A: Type} `{EqGroup A} (x y: QuotFreeGroup A) :
+  to_canon (quot_concat x y) = canon_concat (to_canon x) (to_canon y).
+Proof.
+  destruct x as [x |]; [|auto]. cbn. induction x as [b' v' | v' p x' | v' x']; cbn.
+  - apply quot_canon_cons_homomorphism.
+  - destruct (to_canon' x') as [[b v] l] eqn:c.
+    assert (hd_eq : quot_hd' x' = (b, v)).
+    { apply some_eq. rewrite quot_canon_hd. cbn. now rewrite c. }
+    rewrite hd_eq. cbn in *. rewrite <- IHx'. apply quot_canon_cons_homomorphism.
+  - destruct (to_canon' x') as [[b v] l] eqn:c.
+    assert (hd_eq : quot_hd' x' = (b, v)).
+    { apply some_eq. rewrite quot_canon_hd. cbn. now rewrite c. }
+    rewrite hd_eq. cbn in *. rewrite <- IHx'. apply quot_canon_cons_homomorphism.
+Qed.
+
+
+
+
+
+(* Canon concat laws *)
+Fixpoint canon_apinv {A: Type} `{EqGroup A} (x y: CanonFreeGroup A) :=
+  match x with
+  | [] => y
+  | (b, v) :: x' => canon_apinv x' ((negb b, v) :: y)
+  end.
+
+Definition canon_inv {A: Type} `{EqGroup A} (x: CanonFreeGroup A) := canon_apinv x [].
+
+Fixpoint canon_append {A: Type} `{EqGroup A} (b: bool) (v: A) (x: CanonFreeGroup A) :=
+  match x with
+  | [] => [(b, v)]
+  | [(b', v')] => if negb (eqf v v') || eqb b b'
+                     then [(b', v'); (b, v)]
+                     else []
+  | h :: x' => h :: (canon_append b v x')
+  end.
+
+Lemma append_for_normalized {A: Type} `{EqGroup A} (b: bool) (v: A) (x : CanonFreeGroup A) : 
   Normalized (x ++ [(b, v)]) -> x ++ [(b, v)] = canon_append b v x.
 Proof.
-  revert b v. induction x; auto; intros b v H0; destruct a. cbn in *.
-  destruct x.
+  induction x as [|(b' & v')]; [auto|..]; intros H0. cbn in *.
+  destruct x as [| (b'' & v'')].
   - cbn in *. dependent destruction H0. destruct H0.
-    + rewrite <- eqf_false_iff in H0. rewrite eqf_sym, H0. auto.
-    + subst. rewrite eqb_reflx, orb_true_r. auto.
+    + rewrite not_eqf_iff in H0. rewrite eqf_sym, H0. auto.
+    + subst. now  rewrite eqb_reflx, orb_true_r.
   - rewrite IHx; auto. dependent destruction H0; auto.
 Qed.
 
-Lemma cons_for_normalized {A: Type} `{Group A} (b: bool) (v: A) (x : CanonFreeGroup A) : 
+Lemma cons_for_normalized {A: Type} `{EqGroup A} (b: bool) (v: A) (x : CanonFreeGroup A) : 
   Normalized ((b, v) :: x) -> (b, v) :: x = canon_cons b v x.
 Proof.
   intros Nx. destruct x as [| (b' & v')]; auto. cbn. dependent destruction Nx.
-  rewrite condition_iff in H0. rewrite H0. auto.
+  rewrite condition_iff in H0. now rewrite H0.
 Qed.
 
-Lemma canon_cons_inv_elem {A: Type} `{Group A} (b b': bool) (v v': A) (x: CanonFreeGroup A) :
+Lemma canon_cons_inv_elem {A: Type} `{EqGroup A} (b b': bool) (v v': A) (x: CanonFreeGroup A) :
   Normalized x -> negb (eqf v v') || eqb b b' = false -> canon_cons b v (canon_cons b' v' x) = x.
 Proof.
   intros Nx H0. induction Nx as [| b'' v'' | b'' b''' v'' v'''].
   - cbn. rewrite H0. auto.
   - cbn. destruct (negb (eqf v' v'') || eqb b' b'') eqn:H1.
-    + cbn. rewrite H0. auto.
+    + cbn. now rewrite H0.
     + cbn. rewrite orb_false_iff, negb_false_iff in H0, H1. destruct H0, H1.
-      rewrite eqf_true_iff in H0. rewrite eqf_true_iff in H1. subst. f_equal. f_equal.
+      rewrite <-eqf_iff in H0. rewrite <-eqf_iff in H1. subst. f_equal. f_equal.
       apply eqb_false_chain with (y := b'); auto.
   - rewrite condition_iff in H1. cbn. destruct (negb (eqf v' v'') || eqb b' b'') eqn:H2.
     + cbn. rewrite H0. auto.
@@ -546,15 +507,7 @@ Proof.
       destruct H0, H2. subst. rewrite negb_involutive, H1. auto.
 Qed.
 
-Lemma normalized_without_head {A: Type} `{Group A} (b: bool) (v: A) (x: CanonFreeGroup A) :
-  Normalized ((b, v) :: x) -> Normalized x.
-Proof.
-  intros Nx. destruct x.
-  - constructor.
-  - destruct p as (b', v'). dependent destruction Nx. auto.
-Qed.
-
-Lemma canon_concat_cons {A: Type} `{Group A} (b: bool) (v: A) (x y: CanonFreeGroup A) :
+Lemma canon_concat_cons {A: Type} `{EqGroup A} (b: bool) (v: A) (x y: CanonFreeGroup A) :
   Normalized x -> Normalized y -> canon_concat (canon_cons b v x) y  = canon_cons b v (canon_concat x y).
 Proof.
   intros Nx Ny. destruct x as [| (b' & v') x']; auto. cbn. 
@@ -563,7 +516,7 @@ Proof.
   apply (normalized_without_head b' v'). auto.
 Qed.
 
-Theorem canon_concat_assoc {A: Type} `{Group A} (x y z: CanonFreeGroup A) : Normalized x -> 
+Theorem canon_concat_assoc {A: Type} `{EqGroup A} (x y z: CanonFreeGroup A) : Normalized x -> 
    Normalized y -> Normalized z -> canon_concat (canon_concat x y) z = canon_concat x (canon_concat y z).
 Proof.
   revert y z. induction x; intros y z Nx Ny Nz; auto. cbn. destruct a. 
@@ -572,351 +525,92 @@ Proof.
   - apply concat_norm; auto. apply (normalized_without_head b a). auto.
 Qed.
 
-Lemma normalized_head {A: Type} `{Group A} (b: bool) (v: A) (x: CanonFreeGroup A) :
+Lemma normalized_head {A: Type} `{EqGroup A} (b: bool) (v: A) (x: CanonFreeGroup A) :
   hd_error x = None \/ (exists (b' : bool) (v' : A), hd_error x = Some (b', v') /\ (v <> v' \/ b = b'))
    -> Normalized x -> Normalized ((b, v) :: x).
 Proof.
-  intros H0 Nx. destruct x as [| (b'' & v'')].
-  - constructor.
-  - constructor; auto. destruct H0.
-    + cbn in H0. inversion H0.
-    + cbn in H0. destruct H0 as [b' (v' & (H0 & H1))]. inversion H0. subst. auto.
+  intros H0 Nx. destruct x as [| (b'' & v'')]; constructor; [|auto].
+  destruct H0.
+  - cbn in H0. inversion H0.
+  - cbn in H0. destruct H0 as [b' (v' & (H0 & H1))]. inversion H0. subst. auto.
 Qed.
   
 
-Lemma noramlized_singl_append {A: Type} `{Group A} (b0 b1 b': bool) (v0 v1 v': A) (x: CanonFreeGroup A) :
+Lemma noramlized_singl_append {A: Type} `{EqGroup A} (b0 b1 b': bool) (v0 v1 v': A) (x: CanonFreeGroup A) :
   Normalized ((b0, v0) :: (b1, v1) :: x) -> canon_concat ((b0, v0) :: (b1, v1) :: x) [(b', v')] 
   = (b0, v0) :: canon_concat ((b1, v1) :: x) [(b', v')].
 Proof.
-  revert b0 b1 v0 v1. induction x as [| (b2 & v2)]; intros b0 b1 v0 v1 Nx. 
-  - cbn. dependent destruction Nx. destruct ( negb (eqf v1 v') || eqb b1 b') eqn:e; auto.
-    cbn. rewrite condition_iff in H0. rewrite H0. auto.
-  - cbn in *. dependent destruction Nx. rewrite IHx; auto. rewrite condition_iff in H0.
-    cbn. rewrite H0. auto.
+  revert b0 b1 v0 v1. induction x as [| (b2 & v2)]; intros b0 b1 v0 v1 Nx; cbn in *. 
+  - dependent destruction Nx. destruct ( negb (eqf v1 v') || eqb b1 b') eqn:e; [|auto].
+    cbn. rewrite condition_iff in H0. now rewrite H0.
+  - dependent destruction Nx. rewrite IHx; [|auto]. rewrite condition_iff in H0.
+    cbn. now rewrite H0.
 Qed.
 
-Lemma append_is_concat_at_end {A: Type} `{Group A} (b: bool) (v: A) (x: CanonFreeGroup A) :
+Lemma append_is_concat_at_end {A: Type} `{EqGroup A} (b: bool) (v: A) (x: CanonFreeGroup A) :
   Normalized x -> canon_append b v x = canon_concat x [(b, v)].
 Proof.
   intros Nx. revert b v. induction Nx as [| b' v' | b' b'' v' v'']; auto; intros b v.
-  - cbn. rewrite eqf_sym, eqb_sym. auto.
+  - cbn. now rewrite eqf_sym, eqb_sym.
   - rewrite noramlized_singl_append. 
     + cbn in *. rewrite IHNx; auto.
     + constructor; auto.
 Qed.
 
-Lemma cons_is_concat_at_start {A: Type} `{Group A} (b: bool) (v: A) (x: CanonFreeGroup A) :
+Lemma cons_is_concat_at_start {A: Type} `{EqGroup A} (b: bool) (v: A) (x: CanonFreeGroup A) :
   canon_cons b v x = canon_concat [(b, v)] x.
 Proof.
-  cbn. auto.
+  auto.
 Qed.
 
-Theorem cons_append_comm {A: Type} `{Group A} (b b': bool) (v v': A) (x: CanonFreeGroup A) :
+Theorem cons_append_comm {A: Type} `{EqGroup A} (b b': bool) (v v': A) (x: CanonFreeGroup A) :
   Normalized x -> canon_cons b v (canon_append b' v' x) = canon_append b' v' (canon_cons b v x).
 Proof.
-  intros Nx. rewrite cons_is_concat_at_start, cons_is_concat_at_start, 
+  intros Nx. rewrite cons_is_concat_at_start, cons_is_concat_at_start,
   append_is_concat_at_end, append_is_concat_at_end, canon_concat_assoc; auto.
   - constructor.
   - constructor.
-  - apply concat_norm; auto; try constructor.
+  - apply concat_norm; [constructor | auto].
 Qed.
 
-Theorem canon_concat_append {A: Type} `{Group A} (b: bool) (v: A) (x y: CanonFreeGroup A) :
+Theorem concat_append {A: Type} `{EqGroup A} (b: bool) (v: A) (x y: CanonFreeGroup A) :
   Normalized x -> Normalized y -> 
   canon_concat x (canon_append b v y) = canon_append b v (canon_concat x y).
 Proof.
-  induction x; auto. intros Nx Ny. cbn. destruct a. rewrite IHx; auto. apply cons_append_comm.
-  - apply concat_norm; auto. apply (normalized_without_head b0 a); auto.
-  - apply (normalized_without_head b0 a); auto.
+  induction x as [|(b' & v')]; [auto|]. intros Nx Ny. cbn. rewrite IHx; 
+  [| now apply (normalized_without_head b' v') |auto]. apply cons_append_comm.
+  apply concat_norm; auto. apply (normalized_without_head b' v'); auto.
 Qed.
 
-Lemma appinv_list_remaining {A: Type} `{Group A} (x y: CanonFreeGroup A) :
+Lemma appinv_concat_elim {A: Type} `{EqGroup A} (x y: CanonFreeGroup A) :
   canon_concat x (canon_apinv x y) = y.
 Proof.
-  revert y. induction x; auto. intros y. cbn. destruct a. rewrite IHx.
-  cbn. rewrite eqf_refl, eqb_negb2. cbn. auto.
+  revert y. induction x as [| (b & v)]; [auto|]. intros y. cbn. rewrite IHx.
+  cbn. rewrite eqf_refl, eqb_negb2. auto.
 Qed.
 
-Theorem canon_right_inv {A: Type} `{Group A} (x : CanonFreeGroup A) : 
+Theorem r_canon_concat_inv {A: Type} `{EqGroup A} (x : CanonFreeGroup A) : 
   canon_concat x (canon_inv x) = [].
 Proof.
-  induction x; auto. cbn. destruct a. rewrite appinv_list_remaining.
-  cbn. rewrite eqf_refl, eqb_negb2. cbn. auto.
+  induction x as [| (b & v)]; [auto|]. cbn. rewrite appinv_concat_elim.
+  cbn. rewrite eqf_refl, eqb_negb2. auto.
 Qed.
 
-Lemma cannon_inv_concat {A: Type} `{Group A} (x y: CanonFreeGroup A) : 
+Lemma apinv_def {A: Type} `{EqGroup A} (x y: CanonFreeGroup A) : 
   canon_apinv x y = canon_inv x ++ y.
 Proof.
-  unfold canon_inv. revert y. induction x; auto; intros y.
-  cbn. destruct a. rewrite IHx, (IHx [(negb b, a)]), <- app_assoc.
-  auto.
+  unfold canon_inv. revert y. induction x as [| (b & v)]; [auto|]. intros y.
+  cbn. now rewrite IHx, (IHx [(negb b, v)]), <- app_assoc.
 Qed.
 
-Lemma cannon_inv_append {A: Type} `{Group A} (b: bool) (v: A) (x : CanonFreeGroup A) : 
+Lemma cannon_inv_append {A: Type} `{EqGroup A} (b: bool) (v: A) (x : CanonFreeGroup A) : 
   canon_inv (x ++ [(b, v)]) = (negb b, v) :: canon_inv x.
 Proof.
-  revert b v. induction x; auto. intros b v. cbn. destruct a.
-  rewrite cannon_inv_concat, IHx, cannon_inv_concat, app_comm_cons. auto.
+  revert b v. induction x as [| (b' & v')]; [auto|]. intros b v. cbn.
+  now rewrite apinv_def, IHx, apinv_def, app_comm_cons.
 Qed.
 
-Lemma concat_normalized_l {A: Type} `{Group A} (x y: CanonFreeGroup A) :
-  Normalized (x ++ y) -> Normalized x.
-Proof.
-  destruct x as [| (b, v)].
-  - constructor.
-  - revert b v. induction x as [| (b', v')]; intros b v H0.
-    + constructor.
-    + dependent destruction H0. constructor; auto.
-Qed.
-
-Lemma concat_normalized_r {A: Type} `{Group A} (x y: CanonFreeGroup A) :
-  Normalized (x ++ y) -> Normalized y.
-Proof.
-  revert y. induction x as [| (b, v)]; intros y.
-  - cbn. auto.
-  - intros H0. apply IHx. rewrite <- app_comm_cons in H0.
-    apply (normalized_without_head b v). auto.
-Qed.
-
-Lemma normalized_list_concat {A: Type} `{Group A} (b b': bool) (v v': A) (x y: CanonFreeGroup A) :
-  Normalized (x ++ [(b, v)]) -> Normalized ((b', v') :: y) ->
-  v <> v' \/ b = b' -> Normalized (x ++ (b, v) :: (b', v') :: y).
-Proof.
-  revert b b' v v' y. induction x using rev_ind; intros b b' v v' y Nx Ny H0.
-  - cbn. constructor; auto.
-  - rewrite <- app_assoc. cbn. destruct x as (b'', v''). apply IHx.
-    + apply (concat_normalized_l (x0 ++ [(b'', v'')]) [(b, v)]). auto.
-    + constructor; auto.
-    + assert (Normalized [(b'', v''); (b, v)]).
-      { apply (concat_normalized_r x0). rewrite <- app_assoc in Nx. auto. }
-      dependent destruction H1. auto.
-Qed. 
-
-Theorem rev_normalized {A: Type} `{Group A} (b b': bool) (v v': A) (x: CanonFreeGroup A) :
-  Normalized (x ++ [(b, v)]) -> v <> v' \/ b = b' -> Normalized (x ++ [(b, v); (b', v')]).
-Proof.
-  revert b b' v v'. destruct x as [| (b'', v'')] using rev_ind ; intros b b' v v' Nx H0.
-  - cbn. constructor; auto. constructor.
-  - apply normalized_list_concat; auto. constructor.
-Qed. 
-
-Theorem inv_norm {A: Type} `{Group A} (x: CanonFreeGroup A) : 
-  Normalized x -> Normalized (canon_inv x).
-Proof.
-  intros Nx. induction Nx.
-  - cbn. constructor.
-  - cbn. constructor.
-  - cbn in *. rewrite cannon_inv_concat in IHNx. rewrite cannon_inv_concat.
-    apply rev_normalized; auto. destruct H0; auto. subst. auto.
-Qed.
-
-Theorem canon_left_inv {A: Type} `{Group A} (x : CanonFreeGroup A) : 
-  Normalized x -> canon_concat (canon_inv x) x = [].
-Proof.
-  induction x using rev_ind; auto. intros N. destruct x.
-  rewrite cannon_inv_append. cbn. rewrite append_for_normalized; auto.
-  assert (Normalized x0). { apply (concat_normalized_l x0 [(b, a)]). auto. }
-  rewrite canon_concat_append, IHx; auto.
-  - cbn. rewrite eqf_refl, eqb_negb1. auto.
-  - apply inv_norm; auto.
-Qed.
-
-Theorem canon_left_id {A: Type} `{Group A} (x : CanonFreeGroup A) : 
-  canon_concat [] x = x.
-Proof.
-  auto.
-Qed.
-
-Theorem canon_right_id {A: Type} `{Group A} (x : CanonFreeGroup A) : 
-  Normalized x -> canon_concat x [] = x.
-Proof.
-  intros Nx. induction x as [| (b, v)]; auto. cbn. rewrite IHx, cons_for_normalized; auto.
-  apply (normalized_without_head b v); auto.
-Qed.
-
-(* Free Group eqdec *)
-
-Fixpoint fg_eq' {A: Type} `{Group A} (x y: NonEmptyFreeGroup A) : bool :=
-  match x, y with
-  | Singl xb xv,    Singl yb yv    => eqb xb yb && eqf xv yv
-  | Switch xr _ x', Switch yr _ y' => eqf xr yr && fg_eq' x' y'
-  | Stay xr x',     Stay yr y'     => eqf xr yr && fg_eq' x' y'
-  | _,              _              => false
-  end.
-
-Definition fg_eq {A: Type} `{Group A} (x y: FreeGroup A) : bool :=
-  match x, y with
-  | None,    None    => true
-  | Some x', Some y' => fg_eq' x' y'
-  | _,       _       => false
-  end.
-
-Theorem fq_eqf_eq {A: Type} `{Group A} (x y: FreeGroup A) : reflect (x = y) (fg_eq x y).
-Proof.
-  apply iff_reflect. split.
-  - intros []. destruct x as [x |]; auto. induction x.
-    + cbn. rewrite eqb_reflx, eqf_refl. auto.
-    + cbn in *. rewrite eqf_refl, IHx. auto.
-    + cbn in *. rewrite eqf_refl, IHx. auto.
-  - intros H0. destruct x as [x |]; destruct y as [y |]; cbn in *; try inversion H0; auto.
-    f_equal. revert H0 H2. intros _. revert y. induction x; intros y H0.
-    + destruct y; cbn in *; try inversion H0. rewrite andb_true_iff in H0.
-      destruct H0. rewrite eqb_true_iff in H0. rewrite eqf_true_iff in H1. 
-      subst. auto.
-    + destruct y; cbn in *; inversion H0. rewrite andb_true_iff in H0.
-      destruct H0. rewrite eqf_true_iff in H0. rewrite andb_true_iff in H2.
-      destruct H2. specialize (IHx y H1). subst. auto.
-    + destruct y; cbn in *; inversion H0. rewrite andb_true_iff in H0.
-      destruct H0. rewrite eqf_true_iff in H0. subst. f_equal. apply IHx.
-      rewrite andb_true_iff in H2. destruct H2. auto.
-Qed.
-
-Definition fg_canon_concat {A: Type} `{Group A} (x y: FreeGroup A) : FreeGroup A :=
-  to_uniq (canon_concat (to_canon x) (to_canon y)).
-
-Definition fg_canon_inv {A: Type} `{Group A} (x: FreeGroup A) : FreeGroup A :=
-  to_uniq (canon_inv (to_canon x)).
-
-
-(* Free Group is Group *)
-Definition fg_zero {A: Type} `{Group A} := None (A := NonEmptyFreeGroup A).
-
-Theorem fq_left_inv {A: Type} `{Group A} (x y: FreeGroup A) : 
-  fg_canon_concat (fg_canon_inv x) x = fg_zero.
-Proof.
-  unfold fg_canon_concat, fg_canon_inv. rewrite canon_epi_free_group.
-  - rewrite canon_left_inv; auto. apply free_group_is_normal.
-  - apply inv_norm. apply free_group_is_normal.
-Qed.
-
-Theorem fq_right_inv {A: Type} `{Group A} (x y: FreeGroup A) : 
-  fg_canon_concat x (fg_canon_inv x) = fg_zero.
-Proof.
-  unfold fg_canon_concat, fg_canon_inv. rewrite canon_epi_free_group.
-  - rewrite canon_right_inv; auto.
-  - apply inv_norm. apply free_group_is_normal.
-Qed.
-
-Theorem fq_left_id {A: Type} `{Group A} (x y: FreeGroup A) : 
-  fg_canon_concat fg_zero x = x.
-Proof.
-  unfold fg_canon_concat, fg_canon_inv. cbn. apply free_group_epi_canon.
-Qed.
-
-Theorem fq_right_id {A: Type} `{Group A} (x y: FreeGroup A) : 
-  fg_canon_concat x fg_zero = x.
-Proof.
-  unfold fg_canon_concat, fg_canon_inv. cbn. rewrite canon_right_id.
-  - apply free_group_epi_canon.
-  - apply free_group_is_normal.
-Qed.
-
-Theorem fq_op_assoc {A: Type} `{Group A} (x y z: FreeGroup A) : 
-  fg_canon_concat (fg_canon_concat x y) z = fg_canon_concat x (fg_canon_concat y z).
-Proof.
-  unfold fg_canon_concat, fg_canon_inv. rewrite canon_epi_free_group, canon_epi_free_group.
-  - rewrite canon_concat_assoc; auto; try apply free_group_is_normal.
-  - apply concat_norm; apply free_group_is_normal.
-  - apply concat_norm; apply free_group_is_normal.
-Qed.
-
-Global Program Instance FreeGroup_is_Group {A: Type} `{Group A} : Group (FreeGroup A) := {
-  zero      := fg_zero;
-  op        := fg_canon_concat;
-  inv       := fg_canon_inv;
-  eqf       := fg_eq;
-}.
-
-Next Obligation. apply fq_left_id; auto. Defined.
-Next Obligation. apply fq_right_id; auto. Defined.
-Next Obligation. apply fq_left_inv; auto. Defined.
-Next Obligation. apply fq_right_inv; auto. Defined.
-Next Obligation. apply fq_op_assoc; auto. Defined.
-Next Obligation. apply fq_eqf_eq; auto. Defined.
-
-
-
-(* Suspicous Integers *)
-Global Program Instance Unit_is_Group : Group unit := {
-  zero      := tt;
-  op        := fun _ _ => tt;
-  inv       := fun _ => tt;
-  eqf       := fun _ _ => true;
-}.
-
-Next Obligation. destruct x; auto. Defined.
-Next Obligation. destruct x; auto. Defined.
-Next Obligation. constructor. destruct x, y. auto. Defined.
-
-Definition Integrals := FreeGroup unit.
-
-Class Monad (M : Type -> Type) := MondadDef {
-  pure       : forall {A : Type}, A -> M A;
-  bind       : forall {A B : Type}, M A -> (A -> M B) -> M B;
-  left_bind  : forall {A B : Type} (f: A -> M B) (x: A), bind (pure x) f = f x; 
-  right_bind : forall {A B : Type} (x: M A), bind x pure = x; 
-  comp_bind  : forall {A B C : Type} (f: B -> M C) (g : A -> M B) (x: M A),
-                 bind (bind x g) f = bind x (fun y => bind (g y) f);
-}.
-
-Definition fg_pure {A: Type} `{Group A} (x: A) := Singl true x.
-
-Definition canon_pure {A: Type} `{Group A} (x: A) := [(true, x)].
-
-Fixpoint canon_bind {A B: Type} `{Group A} `{Group B} (x : CanonFreeGroup A)
-  (f: A -> CanonFreeGroup B) : CanonFreeGroup B :=
-  match x with
-  | [] => []
-  | (b, v) :: x' => if b
-                    then canon_concat (f v) (canon_bind x' f)
-                    else canon_concat (canon_inv (f v)) (canon_bind x' f)
-  end.
-
-Definition fg_bind {A B: Type} `{Group A} `{Group B} (x : FreeGroup A)
-  (f: A -> FreeGroup B) : FreeGroup B :=
-  to_uniq (canon_bind (to_canon x) (fun y => to_canon (f y))).
-
-Theorem bind_norm {A B: Type} `{Group A} `{Group B} (x: CanonFreeGroup A)
-  (f: A -> CanonFreeGroup B) : (forall a: A, Normalized (f a)) -> Normalized (canon_bind x f).
-Proof.
-  intros Nf. induction x as [|(b, v)].
-  - cbn. constructor.
-  - cbn. destruct b.
-    + apply concat_norm; auto.
-    + apply concat_norm; try apply inv_norm; auto.
-Qed.
-
-Theorem canon_bind_cons {A B: Type} `{Group A} `{Group B} (b: bool) (v: A) 
-  (x: CanonFreeGroup A) (f: A -> CanonFreeGroup B) :
-  (forall a: A, Normalized (f a)) -> canon_bind (canon_cons b v x) f = 
-  canon_concat (if b then f v else canon_inv (f v)) (canon_bind x f).
-Proof.
-  intros Nf. destruct x as [| (b', v')].
-  - cbn. destruct b; auto.
-  - cbn. destruct b, b'.
-    + rewrite eqb_reflx, orb_true_r. auto.
-    + destruct (eqf v v') eqn:veq; auto. rewrite eqf_true_iff in veq. subst. 
-      cbn. rewrite <- canon_concat_assoc, canon_right_inv; auto.
-      * apply inv_norm. auto.
-      * apply bind_norm; auto.
-    + destruct (eqf v v') eqn:veq; auto. rewrite eqf_true_iff in veq. subst. 
-      cbn. rewrite <- canon_concat_assoc, canon_left_inv; auto.
-      * apply inv_norm. auto.
-      * apply bind_norm; auto.
-    + rewrite eqb_reflx, orb_true_r. auto.
-Qed.
-
-Theorem canon_bind_concat {A B: Type} `{Group A} `{Group B} (x y : CanonFreeGroup A)
-  (f: A -> CanonFreeGroup B) : (forall a: A, Normalized (f a)) ->
-  canon_bind (canon_concat x y) f = canon_concat (canon_bind x f) (canon_bind y f).
-Proof.
-  intros Nf. induction x as [| (b, v)]; auto. cbn. rewrite canon_bind_cons; auto.
-  destruct b.
-  - rewrite IHx, canon_concat_assoc; try apply bind_norm;auto.
-  - rewrite IHx, canon_concat_assoc; try apply bind_norm; try apply inv_norm; auto.
-Qed.
-
-Lemma concat_for_normalized {A: Type} `{Group A} (x y: CanonFreeGroup A) :
+Lemma concat_for_normalized {A: Type} `{EqGroup A} (x y: CanonFreeGroup A) :
   Normalized (x ++ y) -> canon_concat x y = x ++ y.
 Proof.
   intro N. induction x as [| (b, v)]; auto. cbn. 
@@ -924,134 +618,167 @@ Proof.
   rewrite app_comm_cons. auto. 
 Qed.
 
-Lemma eqb_neg_izo (x y : bool) : eqb (negb x) (negb y) = eqb x y.
+Lemma normalized_list_concat {A: Type} `{EqGroup A} (b b': bool) (v v': A) (x y: CanonFreeGroup A) :
+  Normalized (x ++ [(b, v)]) -> Normalized ((b', v') :: y) ->
+  v <> v' \/ b = b' -> Normalized (x ++ (b, v) :: (b', v') :: y).
 Proof.
-  destruct x, y; auto.
-Qed.
-
-Lemma cons_inv_is_append {A: Type} `{Group A} (b: bool) (v : A) (x: CanonFreeGroup A) :
-  Normalized x -> canon_inv (canon_cons b v x) = canon_append (negb b) v (canon_inv x).
-Proof.
-  intros Nx. induction x as [| (b', v')]; auto. cbn.
-  destruct (negb (eqf v v') || eqb b b') eqn:e.
-  - cbn. assert (Normalized (canon_inv ((b', v') :: x))) by (apply inv_norm; auto).
-    rewrite cannon_inv_concat, cannon_inv_concat, append_is_concat_at_end, 
-    concat_for_normalized, <- app_assoc; auto.
-    + rewrite <- app_assoc. cbn. apply rev_normalized.
-      * rewrite <- cannon_inv_concat. auto.
-      * rewrite condition_iff, eqf_sym, eqb_sym, eqb_neg_izo. auto.
-    + rewrite <- cannon_inv_concat. auto.
-  - assert (Normalized (canon_inv ((b', v') :: x))) by (apply inv_norm; auto).
-    rewrite cannon_inv_concat,  cannon_inv_concat, append_is_concat_at_end, 
-    <- (concat_for_normalized (canon_inv x) [(negb b', v')]), canon_concat_assoc;
-    auto; try constructor.
-    + cbn. rewrite eqf_sym, eqb_sym, eqb_neg_izo, e, canon_right_id, app_nil_r; auto.
-      apply inv_norm. apply (normalized_without_head b' v'). auto.
-    + apply inv_norm. apply (normalized_without_head b' v'). auto.
-    + rewrite <- cannon_inv_concat. auto.
-    + rewrite <- cannon_inv_concat. auto.
-Qed.
-
-Lemma cons_apinv_is_append {A: Type} `{Group A} (b: bool) (v : A) (x: CanonFreeGroup A) :
-  Normalized x -> canon_apinv (canon_cons b v x) [] = canon_append (negb b) v (canon_apinv x []).
-Proof.
-  intros Nx. apply cons_inv_is_append. auto.
+  revert b b' v v' y. induction x using rev_ind; intros b b' v v' y Nx Ny H0.
+  - cbn. constructor; auto.
+  - rewrite <- app_assoc. cbn. destruct x as (b'', v''). apply IHx.
+    + now apply (concat_normalized_l (x0 ++ [(b'', v'')]) [(b, v)]).
+    + constructor; auto.
+    + assert (Normalized [(b'', v''); (b, v)]) by
+      (apply (concat_normalized_r x0); now rewrite <- app_assoc in Nx).
+      dependent destruction H1. auto.
 Qed. 
 
-Lemma canon_concat_inv {A: Type} `{Group A} (x y: CanonFreeGroup A) :
-  Normalized x -> Normalized y -> 
-  canon_inv (canon_concat x y) = canon_concat (canon_inv y) (canon_inv x). 
+Theorem rev_normalized {A: Type} `{EqGroup A} (b b': bool) (v v': A) (x: CanonFreeGroup A) :
+  Normalized (x ++ [(b, v)]) -> v <> v' \/ b = b' -> Normalized (x ++ [(b, v); (b', v')]).
 Proof.
-  unfold canon_inv. intros Nx Ny. induction x as [| (b, v)].
-  - cbn. rewrite canon_right_id; auto. apply inv_norm; auto.
-  - cbn. assert (Normalized x) by (apply (normalized_without_head b v); auto).
-    assert (Normalized (canon_inv ((b, v) :: x))) by (apply inv_norm; auto).
-    rewrite cons_apinv_is_append, IHx, (cannon_inv_concat x [(negb b, v)]), 
-    <- concat_for_normalized, append_is_concat_at_end, canon_concat_assoc; auto; 
-    try constructor; try apply inv_norm; auto.
-    + apply concat_norm;  apply inv_norm; auto. 
-    + rewrite <- cannon_inv_concat. auto.
-    + apply concat_norm; auto.
-Qed.
-
-Lemma canon_concat_apinv {A: Type} `{Group A} (x y: CanonFreeGroup A) :
-  Normalized x -> Normalized y -> 
-  canon_apinv (canon_concat x y) [] = canon_concat (canon_apinv y []) (canon_apinv x []).
-Proof. 
-  intros Hx Hy. apply canon_concat_inv; auto.
-Qed.
-
-Lemma canon_bind_rev {A B: Type} `{Group A} `{Group B} (b: bool) (v: A)
-  (x: CanonFreeGroup A) (f: A -> CanonFreeGroup B) : (forall a: A, Normalized (f a)) -> 
-  (canon_bind (x ++ [(b, v)]) f) = canon_concat (canon_bind x f) (if b then f v else canon_inv (f v)).
-Proof.
-  intros Nf. induction x as [| (b', v')]; auto.
-  - cbn. destruct b; rewrite canon_right_id; auto. apply inv_norm. auto.
-  - cbn. destruct b, b'.
-    + rewrite canon_concat_assoc, IHx; try apply bind_norm; auto.
-    + rewrite canon_concat_assoc, IHx; try apply bind_norm; try apply inv_norm; auto.
-    + rewrite canon_concat_assoc, IHx; try apply bind_norm; try apply inv_norm; auto.
-    + rewrite canon_concat_assoc, IHx; try apply bind_norm; try apply inv_norm; auto.
-Qed.
-
-Lemma concat_inv_inv {A: Type} `{Group A} (x : CanonFreeGroup A) : 
-  Normalized x -> canon_inv (canon_inv x) = x.
-Proof.
-  intro Nx. rewrite <- (canon_right_id (canon_inv (canon_inv x))), <- (canon_left_inv x),
-  <- (canon_concat_assoc), canon_left_inv; try apply inv_norm; try apply inv_norm; auto.
-Qed.
-
-Lemma concat_apinv_apinv {A: Type} `{Group A} (x : CanonFreeGroup A) : 
-  Normalized x -> canon_apinv (canon_apinv x []) [] = x.
-Proof.
-  intro Nx. apply concat_inv_inv. auto.
-Qed.
-
-Theorem canon_bind_inv {A B: Type} `{Group A} `{Group B} (x: CanonFreeGroup A)
-  (f: A -> CanonFreeGroup B) : (forall a: A, Normalized (f a)) -> 
-  canon_inv (canon_bind x f) = (canon_bind (canon_inv x) f).
-Proof.
-  unfold canon_inv. intros Nf. induction x as [| (b, v)]; auto. cbn. destruct b.
-  - cbn. rewrite canon_concat_apinv, IHx, (cannon_inv_concat x [(false, v)]), canon_bind_rev;
-    try apply bind_norm; auto.
-  - cbn. rewrite canon_concat_apinv, IHx, (cannon_inv_concat x [(true, v)]), canon_bind_rev;
-    try apply bind_norm; try apply inv_norm; auto. unfold canon_inv.
-    rewrite concat_apinv_apinv; auto. 
+  revert b b' v v'. destruct x as [| (b'', v'')] using rev_ind ; intros b b' v v' Nx H0.
+  - cbn. constructor; [auto | constructor].
+  - apply normalized_list_concat; [auto | constructor | auto].
 Qed. 
 
-
-
-Theorem canon_comp_bind {A B C : Type} `{Group A} `{Group B} `{Group C}
-  (f: B -> CanonFreeGroup C) (g : A -> CanonFreeGroup B) (x: CanonFreeGroup A) : 
-  (forall b: B, Normalized (f b)) -> (forall a: A, Normalized (g a)) ->
-  canon_bind (canon_bind x g) f = canon_bind x (fun y => canon_bind (g y) f).
+Theorem inv_norm {A: Type} `{EqGroup A} (x: CanonFreeGroup A) : 
+  Normalized x -> Normalized (canon_inv x).
 Proof.
-  intros Nf Ng. induction x as [|(b, v) x]; auto. cbn. destruct b.
-  - rewrite canon_bind_concat, IHx; auto.
-  - rewrite canon_bind_concat, IHx, <- canon_bind_inv; auto.
+  intros Nx. induction Nx; cbn in *; [constructor | constructor |].
+  rewrite apinv_def in IHNx. rewrite apinv_def.
+  apply rev_normalized; auto. destruct H0; auto. subst. auto.
 Qed.
 
-Theorem canon_left_bind {A B : Type} `{Group A} `{Group B} (f : A -> CanonFreeGroup B)
-  (x: A) : (forall a: A, Normalized (f a)) -> canon_bind (canon_pure x) f = f x.
+Theorem l_canon_concat_inv {A: Type} `{EqGroup A} (x : CanonFreeGroup A) : 
+  Normalized x -> canon_concat (canon_inv x) x = [].
 Proof.
-  intro Nf. cbn. rewrite canon_right_id; auto.
+  induction x as [| (b & v)] using rev_ind; [auto|]. intros N.
+  rewrite cannon_inv_append. cbn. rewrite append_for_normalized; auto.
+  assert (Normalized x) by now apply (concat_normalized_l x [(b, v)]).
+  rewrite concat_append, IHx; auto.
+  - cbn. rewrite eqf_refl, eqb_negb1. auto.
+  - apply inv_norm; auto.
 Qed.
 
-Theorem canon_right_bind {A B : Type} `{Group A} `{Group B} (f : A -> CanonFreeGroup B)
-  (x: CanonFreeGroup A) : Normalized x -> canon_bind x canon_pure = x.
+Theorem l_canon_concat_id {A: Type} `{EqGroup A} (x : CanonFreeGroup A) : 
+  canon_concat [] x = x.
 Proof.
-  intro Nx. induction x as [| (b, v)]; auto. cbn. destruct b.
-  - rewrite IHx.
-    + symmetry. apply cons_for_normalized. auto.
-    + apply (normalized_without_head true v). auto.
-  - rewrite IHx.
-    + symmetry. apply cons_for_normalized. auto.
-    + apply (normalized_without_head false v). auto.
+  auto.
 Qed.
-  
-  
+
+Theorem r_canon_concat_id {A: Type} `{EqGroup A} (x : CanonFreeGroup A) : 
+  Normalized x -> canon_concat x [] = x.
+Proof.
+  intros Nx. induction x as [| (b, v)]; [auto|]. cbn. rewrite IHx, cons_for_normalized; auto.
+  apply (normalized_without_head b v); auto.
+Qed.
 
 
 
 
+
+(* Free Group is Group *)
+Definition quot_zero {A: Type} `{EqGroup A} := None (A := NEQuotFreeGroup A).
+
+Definition quot_via_canon_concat {A: Type} `{EqGroup A} (x y: QuotFreeGroup A) : QuotFreeGroup A :=
+  to_quot (canon_concat (to_canon x) (to_canon y)).
+
+Definition quot_via_canon_inv {A: Type} `{EqGroup A} (x: QuotFreeGroup A) : QuotFreeGroup A :=
+  to_quot (canon_inv (to_canon x)).
+
+Theorem l_quot_via_canon_concat_inv {A: Type} `{EqGroup A} (x y: QuotFreeGroup A) : 
+  quot_via_canon_concat (quot_via_canon_inv x) x = quot_zero.
+Proof.
+  unfold quot_via_canon_concat, quot_via_canon_inv. rewrite canon_epi_quot.
+  - rewrite l_canon_concat_inv; auto. apply quot_is_normal.
+  - apply inv_norm. apply quot_is_normal.
+Qed.
+
+Theorem r_quot_via_canon_concat_inv {A: Type} `{EqGroup A} (x y: QuotFreeGroup A) : 
+  quot_via_canon_concat x (quot_via_canon_inv x) = quot_zero.
+Proof.
+  unfold quot_via_canon_concat, quot_via_canon_inv. rewrite canon_epi_quot.
+  - rewrite r_canon_concat_inv; auto.
+  - apply inv_norm. apply quot_is_normal.
+Qed.
+
+Theorem l_quot_via_canon_concat_id {A: Type} `{EqGroup A} (x y: QuotFreeGroup A) : 
+  quot_via_canon_concat quot_zero x = x.
+Proof.
+  unfold quot_via_canon_concat. cbn. apply quot_epi_canon.
+Qed.
+
+Theorem r_quot_via_canon_concat_id {A: Type} `{EqGroup A} (x y: QuotFreeGroup A) : 
+  quot_via_canon_concat x quot_zero = x.
+Proof.
+  unfold quot_via_canon_concat. cbn. rewrite r_canon_concat_id.
+  - apply quot_epi_canon.
+  - apply quot_is_normal.
+Qed.
+
+Theorem quot_via_canon_concat_assoc {A: Type} `{EqGroup A} (x y z: QuotFreeGroup A) : 
+  quot_via_canon_concat (quot_via_canon_concat x y) z = quot_via_canon_concat x (quot_via_canon_concat y z).
+Proof.
+  unfold quot_via_canon_concat. rewrite canon_epi_quot, canon_epi_quot.
+  - rewrite canon_concat_assoc; auto; try apply quot_is_normal.
+  - apply concat_norm; apply quot_is_normal.
+  - apply concat_norm; apply quot_is_normal.
+Qed.
+
+Global Program Instance QuotFreeGroup_is_Group {A: Type} `{EqGroup A} : Group (QuotFreeGroup A) := {
+  zero      := None;
+  op        := quot_via_canon_concat;
+  inv       := quot_via_canon_inv;
+}.
+
+Next Obligation. now apply l_quot_via_canon_concat_id. Defined.
+Next Obligation. now apply r_quot_via_canon_concat_id. Defined.
+Next Obligation. now apply l_quot_via_canon_concat_inv. Defined.
+Next Obligation. now apply r_quot_via_canon_concat_inv. Defined.
+Next Obligation. now apply quot_via_canon_concat_assoc. Defined.
+
+(* Free Group eqdec *)
+
+Fixpoint quot_eq' {A: Type} `{EqGroup A} (x y: NEQuotFreeGroup A) : bool :=
+  match x, y with
+  | Singl xb xv,    Singl yb yv    => eqb xb yb && eqf xv yv
+  | Switch xr _ x', Switch yr _ y' => eqf xr yr && quot_eq' x' y'
+  | Stay xr x',     Stay yr y'     => eqf xr yr && quot_eq' x' y'
+  | _,              _              => false
+  end.
+
+Definition quot_eq {A: Type} `{EqGroup A} (x y: QuotFreeGroup A) : bool :=
+  match x, y with
+  | None,    None    => true
+  | Some x', Some y' => quot_eq' x' y'
+  | _,       _       => false
+  end.
+
+Theorem quot_eqf_eq {A: Type} `{EqGroup A} (x y: QuotFreeGroup A) : reflect (x = y) (quot_eq x y).
+Proof.
+  apply iff_reflect. split.
+  - intros []. destruct x as [x |]; auto. induction x;  cbn in *. 
+    + now rewrite eqb_reflx, eqf_refl.
+    + now rewrite eqf_refl, IHx.
+    + now rewrite eqf_refl, IHx.
+  - intros H0. destruct x as [x |]; destruct y as [y |]; cbn in *; [| inversion H0 | inversion H0 | auto].
+    f_equal. revert H0. revert y. induction x; intros y H0.
+    + destruct y; cbn in *; [| inversion H0 | inversion H0]. 
+      rewrite andb_true_iff in H0; destruct H0. rewrite eqb_true_iff in H0.
+      rewrite <-eqf_iff in H1. subst. auto.
+    + destruct y; cbn in *; [inversion H0 | | inversion H0]. rewrite andb_true_iff in H0.
+      destruct H0. rewrite <-eqf_iff in H0. specialize (IHx y H1). subst. auto.
+    + destruct y; cbn in *; [inversion H0| inversion H0 |]. rewrite andb_true_iff in H0.
+      destruct H0. rewrite <-eqf_iff in H0. specialize (IHx y H1). subst. auto.
+Qed.
+
+
+Global Program Instance QuotFreeGroup_is_EqDec {A: Type} `{EqGroup A} : EqDec (QuotFreeGroup A) := {
+  eqf       := quot_eq;
+}.
+
+Next Obligation. apply quot_eqf_eq; auto. Defined.
+
+
+(* Exotic Integers *)
+Definition FreeGroupIntegrals := QuotFreeGroup unit.
 
