Master/Lib/Algebra.v
@@ -43,6 +43,12 @@ Proof.
   apply group_equation_r_simp with (c := inv y). auto.
 Qed.
 
+Lemma add_is_non_zero {A: Type} `{Group A} (x y : A) : x <> zero -> op x y <> y.
+Proof.
+  intros H0 H1. apply H0. apply group_equation_r_simp with (c := op y (inv y)).
+  rewrite <- op_assoc, H1, r_op_inv, l_op_id. auto.
+Qed.
+
 Lemma group_op_inv {A: Type} `{Group A} (x y: A) : inv (op x y) = op (inv y) (inv x).
 Proof.
   unfold sub. apply group_equation_l_simp with (a := y). 
@@ -51,31 +57,53 @@ Proof.
   rewrite r_op_inv, <- op_assoc, r_op_inv. auto.
 Qed.
 
+Theorem group_inv_inv {A: Type} `{Group A} (x: A) : inv (inv x) = x.
+Proof.
+  rewrite <- (r_op_id (inv (inv x))), <- (l_op_inv x), <- (op_assoc), l_op_inv, l_op_id.
+  auto.
+Qed.
 
-
-
-
-Class Field (A : Type) `{Group A} := FieldDef {
-  one       : A;
-  mul       : A -> A -> A;
-  mul_inv   : A -> A;
-  op_comm   : forall x y: A, op x y = op y x;
-  mul_comm  : forall x y: A, mul x y = mul y x;
-  l_mul_id  : forall x: A, mul one x = x;
-  r_mul_id  : forall x: A, mul x one = x;
-  l_mul_inv : forall x: A, mul (mul_inv x) x = one;
-  r_mul_inv : forall x: A, mul x (mul_inv x) = one;
-  mul_assoc : forall x y z: A, mul (mul x y) z = mul x (mul y z);
-  distr     : forall x y z: A, mul x (op y z) = op (mul x y) (mul x z);
+Global Program Instance Unit_is_Group : Group unit := {
+  zero      := tt;
+  op        := fun _ _ => tt;
+  inv       := fun _ => tt;
 }.
 
-Lemma field_zero_mul_l {A: Type} `{Field A} (x: A) : mul x zero = zero.
+Next Obligation. destruct x; auto. Defined.
+Next Obligation. destruct x; auto. Defined.
+
+
+
+
+
+Class Ring (A : Type) `{Group A} := RingDef {
+  one       : A;
+  mul       : A -> A -> A;
+  op_comm   : forall x y: A, op x y = op y x;
+  l_mul_id  : forall x: A, mul one x = x;
+  r_mul_id  : forall x: A, mul x one = x;
+  mul_assoc : forall x y z: A, mul (mul x y) z = mul x (mul y z);
+  distr_l   : forall x y z: A, mul x (op y z) = op (mul x y) (mul x z);
+  distr_r   : forall x y z: A, mul (op y z) x = op (mul y x) (mul z x);
+}.
+
+Lemma ring_zero_mul_l {A: Type} `{Ring A} (x: A) : mul x zero = zero.
 Proof.
   assert (zero = op (mul x (op zero one)) (inv x)). {
     rewrite l_op_id, r_mul_id, r_op_inv. auto.
   } 
-  rewrite H1 at 2. rewrite distr, r_mul_id, op_assoc, r_op_inv, r_op_id. auto.
+  rewrite H1 at 2. now rewrite distr_l, r_mul_id, op_assoc, r_op_inv, r_op_id.
 Qed.
+
+Lemma ring_zero_mul_r {A: Type} `{Ring A} (x: A) : mul zero x = zero.
+Proof.
+  assert (zero = op (mul (op zero one) x) (inv x)). {
+    rewrite l_op_id, l_mul_id, r_op_inv. auto.
+  } 
+  rewrite H1 at 2. now rewrite distr_r, l_mul_id, op_assoc, r_op_inv, r_op_id.
+Qed.
+
+
 
 
 
