Master/Extras/FullQ.v
@@ -1,0 +1,81 @@
+Require Import Qplus.
+Require Import Integer.
+
+Inductive FullQ :=
+| QPos  : Qplus -> FullQ
+| QZero : FullQ
+| QNeg  : Qplus -> FullQ.
+
+Fixpoint Qplus_inv (q: Qplus) : Qplus :=
+match q with
+| N x => D (Qplus_inv x)
+| One => One
+| D x => N (Qplus_inv x)
+end.
+
+Definition Qinv (q: FullQ) : FullQ :=
+match q with
+| QPos x => QPos (Qplus_inv x)
+| QZero  => QZero
+| QNeg x => QNeg (Qplus_inv x)
+end.
+
+Inductive Positive :=
+| POne : Positive
+| PS   : Positive -> Positive.
+
+Fixpoint to_nat (p: Positive) : nat :=
+match p with
+| POne  => 1
+| PS p' => S (to_nat p')
+end.
+
+Fixpoint to_nat_red (p: Positive) : nat :=
+match p with
+| POne  => 0
+| PS p' => S (to_nat_red p')
+end.
+
+Fixpoint from_nat (p: nat) : Positive :=
+match p with
+| 0    => POne
+| 1    => POne
+| S p' => PS (from_nat p')
+end.
+
+Fixpoint from_nat_red (p: nat) : Positive :=
+match p with
+| 0    => POne
+| S p' => PS (from_nat_red p')
+end.
+
+Definition Q' : Type := Z * Positive.
+
+Definition Q'neg (q: Q') : Q' :=
+  let (n, d) := q in (neg n, d).
+
+Definition Q'inv (q: Q') : Q' :=
+match q with
+| (Pos n, d) => (Pos (to_nat_red d), from_nat_red n)
+| (Zero, d)  => (Zero, d)
+| (Neg n, d) => (Neg (to_nat_red d), from_nat_red n)
+end.
+
+Definition Padd (x y: Positive) : Positive :=
+  from_nat ((to_nat x) + (to_nat y)).
+
+Definition Pmul (x y: Positive) : Positive :=
+  from_nat ((to_nat x) * (to_nat y)).
+
+Definition to_Z (x: Positive) : Z :=
+  Pos (to_nat_red x).
+
+Definition Q'add (x y: Q') : Q' :=
+match x y with
+| (xn, xd), (yn, yd) => (add (mul xn (to_Z yd)) (), Pmul xd yd)
+end.
+
+
+
+
+
